PivotBetree/PivotBetreeSpecRefinement.i.dfy
@@ -28,6 +28,7 @@ module PivotBetreeSpecRefinement {
   import opened Options
   import opened BoundedPivotsLib
   import opened BucketsLib
+  import opened TranslationLib
   import opened KeyType
   import PivotBetreeSpecWFNodes
   import opened BucketMaps
@@ -37,21 +38,26 @@ module PivotBetreeSpecRefinement {
   type Node = B.G.Node
   type PNode = P.G.Node
 
+  type Edge = B.G.Edge
   type Reference = B.G.Reference
   type Buffer = B.G.Buffer
 
-  function IChildren(node: PNode) : (m: imap<Key, Reference>)
+  function IChildren(node: PNode) : (m: imap<Key, Edge>)
   requires (node.children.Some? ==> |node.buckets| == |node.children.value|)
   requires WFPivots(node.pivotTable)
+  requires WFEdges(node.edgeTable, node.pivotTable)
   requires NumBuckets(node.pivotTable) == |node.buckets|
   {
     if node.children.Some? then (
-      imap key:Key | BoundedKey(node.pivotTable, key) :: node.children.value[Route(node.pivotTable, key)]
+      imap key:Key | BoundedKey(node.pivotTable, key) :: 
+        B.G.Edge(
+          TranslateKey(node.pivotTable, node.edgeTable, key),
+          node.children.value[Route(node.pivotTable, key)]
+        )
     ) else (
       imap[]
     )
   }
-
 
   function BucketOptGet(bucket: BucketMap, key: Key) : Message
   {
@@ -95,27 +101,27 @@ module PivotBetreeSpecRefinement {
   function INode(node: PNode) : Node
   requires (node.children.Some? ==> |node.buckets| == |node.children.value|)
   requires WFBucketList(node.buckets, node.pivotTable)
+  requires WFEdges(node.edgeTable, node.pivotTable)
   ensures B.WFNode(INode(node))
   {
     B.G.Node(IChildren(node), IBuffer(node))
   }
 
-
-  predicate ReadOpsBucketsWellMarshalled(readOps: seq<P.Layer>)
+  predicate ReadOpsBucketsWellMarshalled(readOps: seq<P.G.ReadOp>)
   {
     forall i | 0 <= i < |readOps| ::
       forall j | 0 <= j < |readOps[i].node.buckets| ::
         BucketWellMarshalled(readOps[i].node.buckets[j])
   }
 
-  function IReadOp(readOp: P.Layer) : (r: B.G.ReadOp)
+  function IReadOp(readOp: P.G.ReadOp) : (r: B.G.ReadOp)
   requires P.WFNode(readOp.node)
   ensures B.WFNode(r.node)
   {
     B.G.ReadOp(readOp.ref, INode(readOp.node))
   }
 
-  function IReadOps(readOps: seq<P.Layer>) : seq<B.G.ReadOp>
+  function IReadOps(readOps: seq<P.G.ReadOp>) : seq<B.G.ReadOp>
   requires forall i | 0 <= i < |readOps| :: P.WFNode(readOps[i].node)
   ensures |readOps| == |IReadOps(readOps)|
   ensures forall i | 0 <= i < |IReadOps(readOps)| :: B.WFNode(IReadOps(readOps)[i].node)
@@ -124,16 +130,31 @@ module PivotBetreeSpecRefinement {
       IReadOps(readOps[..|readOps|-1]) + [IReadOp(readOps[|readOps|-1])]
   }
 
+  function ILayer(layer: P.Layer) : (l: B.Layer)
+  requires P.WFNode(layer.readOp.node)
+  ensures B.WFNode(l.readOp.node)
+  {
+    B.Layer(B.G.ReadOp(layer.readOp.ref, INode(layer.readOp.node)), layer.currentKey)
+  }
+
+  function ILayers(layers: seq<P.Layer>) : seq<B.Layer>
+  requires forall i | 0 <= i < |layers| :: P.WFNode(layers[i].readOp.node)
+  ensures |layers| == |ILayers(layers)|
+  ensures forall i | 0 <= i < |ILayers(layers)| :: B.WFNode(ILayers(layers)[i].readOp.node)
+  {
+    if |layers| == 0 then [] else ILayers(DropLast(layers)) + [ILayer(Last(layers))]
+  }
+
   function IQuery(q: P.LookupQuery) : B.LookupQuery
   requires P.ValidQuery(q)
   {
-    B.LookupQuery(q.key, q.value, IReadOps(q.lookup))
+    B.LookupQuery(q.key, q.value, ILayers(q.lookup))
   }
 
   function ISuccQuery(q: P.SuccQuery) : B.SuccQuery
   requires P.ValidSuccQuery(q)
   {
-    B.SuccQuery(q.start, q.results, q.end, IReadOps(q.lookup))
+    B.SuccQuery(q.start, q.results, q.end, ILayers(q.lookup))
   }
 
   function IInsertion(ins: P.MessageInsertion) : B.MessageInsertion
@@ -142,24 +163,23 @@ module PivotBetreeSpecRefinement {
     B.MessageInsertion(ins.key, ins.msg, INode(ins.oldroot))
   }
 
-  function MovedKeys(node: PNode, slotIndex: int) : iset<Key>
+  function MovedKeys(node: PNode, slot_idx: int) : iset<Key>
   requires WFPivots(node.pivotTable)
   {
-    iset key | BoundedKey(node.pivotTable, key) && Route(node.pivotTable, key) == slotIndex
+    iset key | BoundedKey(node.pivotTable, key) && Route(node.pivotTable, key) == slot_idx
   }
 
   function FlushedKeys(flush: P.NodeFlush) : iset<Key>
   requires P.ValidFlush(flush)
   {
-    //iset key | BoundedKey(node.pivotTable, key) && Route(node.pivotTable, key) == slotIndex && key in keys
-    iset key | key in flush.parent.buckets[flush.slotIndex].as_map().Keys
-            && key !in flush.newparent.buckets[flush.slotIndex].as_map().Keys
+    iset key | key in flush.parent.buckets[flush.slot_idx].as_map().Keys
+            && key !in flush.newparent.buckets[flush.slot_idx].as_map().Keys
   }
 
   function IFlush(flush: P.NodeFlush) : B.NodeFlush
   requires P.ValidFlush(flush)
   {
-    B.NodeFlush(flush.parentref, INode(flush.parent), INode(flush.newparent), flush.childref, INode(flush.child), flush.newchildref, INode(flush.newchild), MovedKeys(flush.parent, flush.slotIndex), FlushedKeys(flush))
+    B.NodeFlush(flush.parentref, INode(flush.parent), INode(flush.newparent), flush.childref, INode(flush.child), flush.newchildref, INode(flush.newchild), MovedKeys(flush.parent, flush.slot_idx), FlushedKeys(flush))
   }
 
   function IGrow(growth: P.RootGrowth) : B.RootGrowth
@@ -215,6 +235,12 @@ module PivotBetreeSpecRefinement {
     )
   }
 
+  function IClone(clone: P.NodeClone) : B.Clone
+  requires P.ValidClone(clone)
+  {
+    B.Clone(INode(clone.oldroot), INode(clone.newroot), P.CloneMap(clone.from, clone.to))
+  }
+
   function IStep(betreeStep: P.BetreeStep) : B.BetreeStep
   requires !betreeStep.BetreeRepivot?
   requires P.ValidBetreeStep(betreeStep)
@@ -237,42 +263,43 @@ module PivotBetreeSpecRefinement {
         assert P.InvNode(P.BetreeStepReads(betreeStep)[2].node);
         B.BetreeRedirect(IMerge(fusion))
       )
+      case BetreeClone(clone) => (
+        B.BetreeClone(IClone(clone))
+      )
     }
   }
 
   lemma RefinesLookup(lookup: P.Lookup, key: Key)
   requires P.WFLookupForKey(lookup, key)
-  ensures B.WFLookupForKey(IReadOps(lookup), key)
+  ensures B.WFLookupForKey(ILayers(lookup), key)
   {
     if (|lookup| == 1) {
     } else {
-      forall idx | P.ValidLayerIndex(DropLast(lookup), idx) && idx < |DropLast(lookup)| - 1
-      ensures P.LookupFollowsChildRefAtLayer(key, DropLast(lookup), idx)
+      var lookup' := DropLast(lookup);
+
+      forall idx | P.ValidLayerIndex(lookup' , idx) && idx < |lookup' | - 1
+      ensures P.LookupFollowsChildRefAtLayer(lookup' , idx)
+      ensures P.LookupFollowsChildEdgeAtLayer(lookup', idx)
       {
-        assert P.LookupFollowsChildRefAtLayer(key, lookup, idx);
-        //assert DropLast(lookup)[idx] == lookup[idx];
-        //assert DropLast(lookup)[idx+1] == lookup[idx+1];
+        assert P.LookupFollowsChildRefAtLayer(lookup, idx);
+        assert P.LookupFollowsChildEdgeAtLayer(lookup, idx);
       }
-      RefinesLookup(DropLast(lookup), key);
-      forall idx | B.ValidLayerIndex(IReadOps(lookup), idx) && idx < |IReadOps(lookup)| - 1
-      ensures key in IReadOps(lookup)[idx].node.children
-      ensures B.LookupFollowsChildRefAtLayer(key, IReadOps(lookup), idx)
+
+      RefinesLookup(lookup', key);
+
+      forall idx | B.ValidLayerIndex(ILayers(lookup), idx) && idx < |ILayers(lookup)| - 1
+      ensures B.LookupFollowsChildRefAtLayer(ILayers(lookup), idx)
+      ensures B.LookupFollowsEdgeAtLayer(ILayers(lookup), idx)
       {
         if idx < |lookup| - 2 {
-          assert B.LookupFollowsChildRefAtLayer(key, IReadOps(DropLast(lookup)), idx);
-          assert key in IReadOps(DropLast(lookup))[idx].node.children;
-          //assert key in IReadOps(lookup)[idx].node.children;
-          assert B.LookupFollowsChildRefAtLayer(key, IReadOps(lookup), idx);
+          assert B.LookupFollowsChildRefAtLayer(ILayers(lookup'), idx);
+          assert B.LookupFollowsEdgeAtLayer(ILayers(lookup'), idx);
+
+          assert B.LookupFollowsChildRefAtLayer(ILayers(lookup), idx);
+          assert B.LookupFollowsEdgeAtLayer(ILayers(lookup), idx);
         } else {
-          assert P.LookupFollowsChildRefAtLayer(key, lookup, |lookup|-2);
-          /*
-          assert lookup[|lookup|-2].node.children.Some?;
-          assert key in IChildren(lookup[|lookup|-2].node);
-          assert key in INode(lookup[|lookup|-2].node).children;
-          assert key in IReadOp(lookup[|lookup|-2]).node.children;
-          assert key in IReadOps(lookup)[idx].node.children;
-          assert B.LookupFollowsChildRefAtLayer(key, IReadOps(lookup), idx);
-          */
+          assert P.LookupFollowsChildRefAtLayer(lookup, |lookup|-2);
+          assert P.LookupFollowsChildEdgeAtLayer(lookup, |lookup|-2);
         }
       }
     }
@@ -280,10 +307,10 @@ module PivotBetreeSpecRefinement {
 
   lemma RefinesInterpretLookup(lookup: P.Lookup, key: Key)
   requires P.WFLookupForKey(lookup, key)
-  requires Last(lookup).node.children.Some?
-  ensures B.WFLookupForKey(IReadOps(lookup), key)
-  ensures P.LookupVisitsWellMarshalledBuckets(lookup, key) ==>
-    B.InterpretLookup(IReadOps(lookup), key) == P.InterpretLookup(lookup, key)
+  requires Last(lookup).readOp.node.children.Some?
+  ensures B.WFLookupForKey(ILayers(lookup), key)
+  ensures P.LookupVisitsWellMarshalledBuckets(lookup) ==>
+    B.InterpretLookup(ILayers(lookup)) == P.InterpretLookup(lookup)
   {
     RefinesLookup(lookup, key);
 
@@ -299,66 +326,67 @@ module PivotBetreeSpecRefinement {
           == P.InterpretLookup(lookup, key);
       */
     } else {
-      forall idx | P.ValidLayerIndex(DropLast(lookup), idx) && idx < |DropLast(lookup)| - 1
-      ensures P.LookupFollowsChildRefAtLayer(key, DropLast(lookup), idx)
+      var lookup' := DropLast(lookup);
+
+      forall idx | P.ValidLayerIndex(lookup', idx) && idx < |lookup'| - 1
+      ensures P.LookupFollowsChildRefAtLayer(lookup', idx)
+      ensures P.LookupFollowsChildEdgeAtLayer(lookup', idx)
       {
-        assert P.LookupFollowsChildRefAtLayer(key, lookup, idx);
+        assert P.LookupFollowsChildRefAtLayer(lookup, idx);
+        assert P.LookupFollowsChildEdgeAtLayer(lookup, idx);
       }
 
-      assert P.LookupFollowsChildRefAtLayer(key, lookup, |lookup|-2);
+      assert P.LookupFollowsChildRefAtLayer(lookup, |lookup|-2);
       RefinesInterpretLookup(DropLast(lookup), key);
-      if P.LookupVisitsWellMarshalledBuckets(lookup, key) {
-        assert B.InterpretLookup(IReadOps(lookup), key) == P.InterpretLookup(lookup, key);
+
+      if P.LookupVisitsWellMarshalledBuckets(lookup) {
+        assert B.InterpretLookup(ILayers(lookup)) == P.InterpretLookup(lookup);
       }
     }
   }
 
   lemma RefinesInterpretLookupAccountingForLeaf(lookup: P.Lookup, key: Key, value: Value)
   requires P.WFLookupForKey(lookup, key)
-  ensures B.WFLookupForKey(IReadOps(lookup), key)
-  ensures P.LookupVisitsWellMarshalledBuckets(lookup, key) ==>
-      B.InterpretLookup(IReadOps(lookup), key) == P.InterpretLookupAccountingForLeaf(lookup, key)
+  ensures B.WFLookupForKey(ILayers(lookup), key)
+  ensures P.LookupVisitsWellMarshalledBuckets(lookup) ==>
+      B.InterpretLookup(ILayers(lookup)) == P.InterpretLookupAccountingForLeaf(lookup)
   {
     RefinesLookup(lookup, key);
 
-    if (Last(lookup).node.children.Some?) {
+    if (Last(lookup).readOp.node.children.Some?) {
       RefinesInterpretLookup(lookup, key);
     } else {
       if |lookup| == 1 {
-        if P.LookupVisitsWellMarshalledBuckets(lookup, key) {
+        if P.LookupVisitsWellMarshalledBuckets(lookup) {
           MergeIsAssociative(
               Update(NopDelta()),
-              P.NodeLookup(lookup[0].node, key),
+              P.NodeLookup(lookup[0].readOp.node, key),
               DefineDefault());
-          assert B.InterpretLookup(IReadOps(lookup), key)
-              //== M.Merge(M.Update(M.NopDelta()), M.Merge(P.NodeLookup(lookup[0].node, key), M.DefineDefault()))
-              //== M.Merge(M.Merge(M.Update(M.NopDelta()), P.NodeLookup(lookup[0].node, key)), DefineDefault())
-              == Merge(P.InterpretLookup(lookup, key), DefineDefault())
-              == P.InterpretLookupAccountingForLeaf(lookup, key);
+          assert B.InterpretLookup(ILayers(lookup))
+              == Merge(P.InterpretLookup(lookup), DefineDefault())
+              == P.InterpretLookupAccountingForLeaf(lookup);
         }
       } else {
-        forall idx | P.ValidLayerIndex(DropLast(lookup), idx) && idx < |DropLast(lookup)| - 1
-        ensures P.LookupFollowsChildRefAtLayer(key, DropLast(lookup), idx)
+        var lookup' := DropLast(lookup);
+
+        forall idx | P.ValidLayerIndex(lookup', idx) && idx < |lookup'| - 1
+        ensures P.LookupFollowsChildRefAtLayer(lookup', idx)
+        ensures P.LookupFollowsChildEdgeAtLayer(lookup', idx)
         {
-          assert P.LookupFollowsChildRefAtLayer(key, lookup, idx);
+          assert P.LookupFollowsChildRefAtLayer(lookup, idx);
+          assert P.LookupFollowsChildEdgeAtLayer(lookup, idx);
         }
 
-        assert P.LookupFollowsChildRefAtLayer(key, lookup, |lookup|-2);
-        RefinesInterpretLookup(DropLast(lookup), key);
+        assert P.LookupFollowsChildRefAtLayer(lookup, |lookup|-2);
+        assert P.LookupFollowsChildEdgeAtLayer(lookup, |lookup|-2);
+        RefinesInterpretLookup(lookup', key);
 
-        if P.LookupVisitsWellMarshalledBuckets(lookup, key) {
+        if P.LookupVisitsWellMarshalledBuckets(lookup) {
           MergeIsAssociative(
-              B.InterpretLookup(DropLast(IReadOps(lookup)), key),
-              P.NodeLookup(Last(lookup).node, key),
+              B.InterpretLookup(DropLast(ILayers(lookup))),
+              P.NodeLookup(Last(lookup).readOp.node, Last(lookup).currentKey),
               DefineDefault());
         }
-            /*
-        assert B.InterpretLookup(IReadOps(lookup), key)
-            == Merge(B.InterpretLookup(DropLast(IReadOps(lookup)), key), Last(IReadOps(lookup)).node.buffer[key])
-            == Merge(B.InterpretLookup(DropLast(IReadOps(lookup)), key), Merge(P.NodeLookup(Last(lookup).node, key), DefineDefault()))
-            == Merge(Merge(B.InterpretLookup(DropLast(IReadOps(lookup)), key), P.NodeLookup(Last(lookup).node, key)), DefineDefault())
-            == P.InterpretLookupAccountingForLeaf(lookup, key);
-            */
       }
     }
   }
@@ -370,27 +398,23 @@ module PivotBetreeSpecRefinement {
   {
     RefinesLookup(q.lookup, q.key);
     RefinesInterpretLookupAccountingForLeaf(q.lookup, q.key, q.value);
-    assert P.LookupVisitsWellMarshalledBuckets(q.lookup, q.key);
+    assert P.LookupVisitsWellMarshalledBuckets(q.lookup);
   }
 
-  lemma KeyWithinUpperBoundIsWithinLookup(
-      lookup: P.Lookup, startKey: Key, key: Key, idx: int)
-  requires P.LookupVisitsWFNodes(lookup)
-  requires P.LookupBoundedKey(startKey, lookup)
-  requires 0 <= idx < |lookup|
-  requires var lookupUpperBound := P.LookupUpperBound(lookup, startKey);
-    && (lookupUpperBound.Some? ==> P.G.Keyspace.lt(key, lookupUpperBound.value))
-  ensures var r := Route(lookup[idx].node.pivotTable, startKey);
-      && Keyspace.lt(KeyToElement(key), lookup[idx].node.pivotTable[r+1])
+  lemma SameILayersReadOp(lookup: P.Lookup, lookup': P.Lookup)
+  requires |lookup| == |lookup'|
+  requires forall i | 0 <= i < |lookup| :: 
+    && P.WFNode(lookup[i].readOp.node)
+    && lookup[i].readOp == lookup'[i].readOp
+  ensures forall i | 0 <= i < |lookup| ::
+    && ILayers(lookup)[i].readOp == ILayers(lookup')[i].readOp 
   {
-    P.reveal_LookupUpperBound();
-    if idx == |lookup| - 1 {
-    } else {
-      KeyWithinUpperBoundIsWithinLookup(DropLast(lookup), startKey, key, idx);
+    if |lookup| > 0 {
+      SameILayersReadOp(DropLast(lookup), DropLast(lookup'));
     }
   }
 
-  lemma InUpperBoundAndNot(a: Key, end: MS.UI.RangeEnd, b: Key)
+  lemma InUpperBoundAndNot(a: Key, end: MS.UI.RangeEnd, b: Key) 
   requires MS.UpperBound(a, end)
   requires !MS.UpperBound(b, end)
   ensures P.G.Keyspace.lt(a, b)
@@ -408,68 +432,241 @@ module PivotBetreeSpecRefinement {
     }
   }
 
-  lemma InRangeImpliesSameRoute(start: MS.UI.RangeStart, key: Key, end: MS.UI.RangeEnd, lookup: P.Lookup, idx: int)
-  requires MS.InRange(start, key, end)
+  lemma LookupUpperBoundLte(lookup: P.Lookup, tt: TranslationTable, targetidx: int)
+  requires 0 <= targetidx < |lookup|
   requires P.LookupVisitsWFNodes(lookup)
-  requires
-    var startKey := if start.NegativeInf? then [] else start.key;
-    && P.LookupBoundedKey(startKey, lookup)
-  requires
-    var startKey := if start.NegativeInf? then [] else start.key;
-    var lookupUpperBound := P.LookupUpperBound(lookup, startKey);
-    && P.WFLookupForKey(lookup, startKey)
-    && (lookupUpperBound.Some? ==> !MS.UpperBound(lookupUpperBound.value, end))
-  requires 0 <= idx < |lookup|
-  ensures BoundedKey(lookup[idx].node.pivotTable, key)
-  ensures var startKey := if start.NegativeInf? then [] else start.key;
-        Route(lookup[idx].node.pivotTable, startKey)
-     == Route(lookup[idx].node.pivotTable, key) // don't know about bounded key
+  requires P.LookupBoundedKey(lookup)
+  requires |lookup| > 0 ==> P.ValidTranslationTable(lookup, tt, 0)
+  ensures 
+    var upperbound := P.LookupUpperBound(lookup, tt);
+    var pset := if targetidx-1 < 0 then None else tt[targetidx-1];
+    var upper := P.LookupUpperBoundAtLayer(lookup[targetidx], pset, lookup[0].currentKey);
+    && (upperbound.None? ==> upper.None?)
+    && (upper.Some? ==> upperbound.Some?)
+    && (upper.Some? ==> P.G.Keyspace.lte(upperbound.value, upper.value))
+  decreases |lookup|
   {
-    var startKey := if start.NegativeInf? then [] else start.key;
-
-    var r := Route(lookup[idx].node.pivotTable, startKey);
-    //assert r > 0 ==> Keyspace.lte(lookup[idx].node.pivotTable[r-1], startKey);
-
-    P.G.Keyspace.EmptyLte(key);
-    //assert Keyspace.lte([], key);
-    //assert Keyspace.lte(startKey, key);
-
-    assert MS.InRange(start, key, end);
-    var lookupUpperBound := P.LookupUpperBound(lookup, startKey);
-    //assert lookupUpperBound.Some? ==> !MS.UpperBound(lookupUpperBound.value, end);
-    //assert MS.UpperBound(key, end);
-    if (lookupUpperBound.Some?) {
-      InUpperBoundAndNot(key, end, lookupUpperBound.value);
+    P.reveal_LookupUpperBound();
+    if |lookup| == targetidx+1 {
+    } else {
+      LookupUpperBoundLte(DropLast(lookup), DropLast(tt), targetidx);
     }
-    //assert lookupUpperBound.Some? ==> Keyspace.lt(key, lookupUpperBound.value);
-    KeyWithinUpperBoundIsWithinLookup(lookup, startKey, key, idx);
-    //assert r < |lookup[idx].node.pivotTable| ==> Keyspace.lt(q.key, lookup[idx].node.pivotTable[r]);
-    RouteIs(lookup[idx].node.pivotTable, key, r);
   }
 
-  lemma InRangeImpliesValidLookup(start: MS.UI.RangeStart, key: Key, end: MS.UI.RangeEnd, lookup: P.Lookup)
-  requires MS.InRange(start, key, end)
+  lemma KeyWithinUpperBoundIsWithinLookup(key: Key, upperbound: Option<Key>, lookup: P.Lookup, tt: TranslationTable, idx: int)
+  requires 0 <= idx < |lookup|
   requires P.LookupVisitsWFNodes(lookup)
+  requires P.LookupBoundedKey(lookup)
+  requires P.ValidTranslationTable(lookup, tt, 0)
+  requires P.G.Keyspace.lte(lookup[0].currentKey, key)
+  requires upperbound == P.LookupUpperBound(lookup, tt)
+  requires upperbound.Some? ==> P.G.Keyspace.lt(key, upperbound.value)
+  ensures idx > 0 && tt[idx-1].Some? ==> IsPrefix(tt[idx-1].value.newPrefix, key)
+  ensures var r := Route(lookup[idx].readOp.node.pivotTable, lookup[idx].currentKey);
+    var currentkey := GenerateKeyAtLayer(key, tt, idx);
+    && Keyspace.lt(KeyToElement(currentkey), lookup[idx].readOp.node.pivotTable[r+1])
+  {
+    P.reveal_LookupUpperBound();
+
+    var pivots := lookup[idx].readOp.node.pivotTable;
+    var r := Route(pivots, lookup[idx].currentKey);
+    var currentkey := GenerateKeyAtLayer(key, tt, idx);
+
+    LookupUpperBoundLte(lookup, tt, idx);
+    if idx > 0 && tt[idx-1].Some? {
+      TranslatePivotPairRangeProperty(KeyToElement(lookup[idx].currentKey),
+          pivots[r+1], tt[idx-1].value.prefix, tt[idx-1].value.newPrefix);
+    }
+  }
+
+  function GenerateKeyAtLayer(key: Key, tt: TranslationTable, idx: int) : (k: Key)
+  requires 0 <= idx <= |tt|
+  {
+    if idx > 0 && tt[idx-1].Some? && IsPrefix(tt[idx-1].value.newPrefix, key)
+    then ApplyPrefixSet(RevPrefixSet(tt[idx-1]), key)
+    else ApplyPrefixSet(None, key)
+  }
+
+  function GenerateLookup(lookup: P.Lookup, key: Key, tt: TranslationTable, idx: int) : (lookup': P.Lookup)
+  requires 0 <= idx < |lookup|
+  requires P.LookupVisitsWFNodes(lookup)
+  requires P.LookupBoundedKey(lookup)
+  requires P.ValidTranslationTable(lookup, tt, 0)
+  ensures |lookup| == |lookup'| + idx
+  ensures forall i | 0 <= i < |lookup'| :: 
+    && lookup'[i].readOp == lookup[i+idx].readOp
+    && lookup'[i].currentKey == GenerateKeyAtLayer(key, tt, i+idx)
+  decreases |lookup| - idx
+  {
+    var currentkey := GenerateKeyAtLayer(key, tt, idx);
+    if idx == |lookup|-1 then (
+      [ P.Layer(lookup[idx].readOp, currentkey) ]
+    ) else (
+      [ P.Layer(lookup[idx].readOp, currentkey) ] +  GenerateLookup(lookup, key, tt, idx+1)
+    )
+  }
+  
+  lemma InRangeImpliesSameRoute(start: MS.UI.RangeStart, key: Key, end: MS.UI.RangeEnd, 
+    lookup: P.Lookup, tt: TranslationTable, lookup': P.Lookup, idx: int)
+  requires MS.InRange(start, key, end)
+  requires P.ValidLayerIndex(lookup, idx)
+  requires P.LookupVisitsWFNodes(lookup)
+  requires P.LookupBoundedKey(lookup)
+  requires lookup[0].currentKey == if start.NegativeInf? then [] else start.key
+  requires P.ValidTranslationTable(lookup, tt, 0)
+  requires lookup' == GenerateLookup(lookup, key, tt, 0)
   requires
-    var startKey := if start.NegativeInf? then [] else start.key;
-    && P.LookupBoundedKey(startKey, lookup)
-  requires
-    var startKey := if start.NegativeInf? then [] else start.key;
-    var lookupUpperBound := P.LookupUpperBound(lookup, startKey);
-    && P.WFLookupForKey(lookup, startKey)
+    var lookupUpperBound := P.LookupUpperBound(lookup, tt);
     && (lookupUpperBound.Some? ==> !MS.UpperBound(lookupUpperBound.value, end))
-  ensures P.WFLookupForKey(lookup, key)
+  ensures idx > 0 && tt[idx-1].Some? ==> IsPrefix(tt[idx-1].value.newPrefix, key)
+  ensures BoundedKey(lookup'[idx].readOp.node.pivotTable, lookup'[idx].currentKey)
+  ensures Route(lookup[idx].readOp.node.pivotTable, lookup[idx].currentKey)
+    == Route(lookup'[idx].readOp.node.pivotTable, lookup'[idx].currentKey)
+  ensures P.G.Keyspace.lte(lookup[idx].currentKey, lookup'[idx].currentKey)
+  ensures var r := Route(lookup[idx].readOp.node.pivotTable, lookup[idx].currentKey);
+    && (BucketWellMarshalled(lookup[idx].readOp.node.buckets[r]) ==> 
+        BucketWellMarshalled(lookup'[idx].readOp.node.buckets[r]))
   {
     var startKey := if start.NegativeInf? then [] else start.key;
+    var pivots := lookup'[idx].readOp.node.pivotTable;
+    var edges := lookup'[idx].readOp.node.edgeTable;
+    var r := Route(pivots, lookup[idx].currentKey);
 
-    forall idx | P.ValidLayerIndex(lookup, idx) && idx < |lookup| - 1 
-    ensures P.LookupFollowsChildRefAtLayer(key, lookup, idx)
-    ensures BoundedKey(lookup[idx].node.pivotTable, key)
-    {
-      assert P.LookupFollowsChildRefAtLayer(startKey, lookup, idx);
-      InRangeImpliesSameRoute(start, key, end, lookup, idx);
+    var upperbound := P.LookupUpperBound(lookup, tt);
+    if upperbound.Some? {
+      InUpperBoundAndNot(key, end, upperbound.value);
     }
-    InRangeImpliesSameRoute(start, key, end, lookup, |lookup|-1);
+
+    P.G.Keyspace.EmptyLte(key);
+    KeyWithinUpperBoundIsWithinLookup(key, upperbound, lookup, tt, idx);
+    assert idx > 0 && tt[idx-1].Some? ==> IsPrefix(tt[idx-1].value.newPrefix, key);
+
+    if  idx > 0 && tt[idx-1].Some? {
+      assert IsPrefix(tt[idx-1].value.newPrefix, key);
+      assert IsPrefix(tt[idx-1].value.newPrefix, startKey) by { reveal_IsPrefix(); }
+
+      assert IsPrefix(tt[idx-1].value.prefix, lookup'[idx].currentKey) by { reveal_IsPrefix(); }
+      assert IsPrefix(tt[idx-1].value.prefix, lookup[idx].currentKey);
+
+      PrefixLteProperties( tt[idx-1].value.newPrefix, startKey, key);
+      PrefixLteProperties( tt[idx-1].value.prefix, lookup[idx].currentKey, lookup'[idx].currentKey);
+    } else {
+      assert lookup[idx].currentKey == startKey;
+      assert lookup'[idx].currentKey == key;
+    }
+    assert P.G.Keyspace.lte(lookup[idx].currentKey, lookup'[idx].currentKey);
+    RouteIs(pivots, lookup'[idx].currentKey, r);
+  }
+
+  predicate LookupConditions(lookup: P.Lookup)
+  {
+    && P.LookupVisitsWFNodes(lookup)
+    && P.LookupBoundedKey(lookup)
+    && P.LookupFollowsChildRefs(lookup)
+    && P.LookupFollowsChildEdges(lookup)
+  }
+
+  lemma {:timeLimitMultiplier 8} WFGenerateLookupIter(start: MS.UI.RangeStart, key: Key, end: MS.UI.RangeEnd,
+    lookup: P.Lookup, lookup': P.Lookup, tt: TranslationTable, idx: int)
+  requires MS.InRange(start, key, end)
+  requires P.ValidLayerIndex(lookup, idx)
+  requires
+    var startKey := if start.NegativeInf? then [] else start.key;
+    && P.WFLookupForKey(lookup, startKey)
+  requires tt == P.LookupTranslationTable(lookup, 0, None)
+  requires lookup' == GenerateLookup(lookup, key, tt, 0)
+  requires
+    var lookupUpperBound := P.LookupUpperBound(lookup, tt);
+    && (lookupUpperBound.Some? ==> !MS.UpperBound(lookupUpperBound.value, end))
+  requires var pset := if idx == 0 then None else tt[idx-1];
+    && tt[idx..] == P.LookupTranslationTable(lookup, idx, pset)
+  ensures LookupConditions(lookup'[idx..])
+  decreases |lookup'| - idx 
+  {
+    var pivots := lookup'[idx].readOp.node.pivotTable;
+    var edges := lookup'[idx].readOp.node.edgeTable;
+    InRangeImpliesSameRoute(start, key, end, lookup, tt, lookup', idx);
+
+    if idx < |lookup'| - 1 {
+      WFGenerateLookupIter(start, key, end, lookup, lookup', tt, idx + 1); 
+      assert P.LookupFollowsChildRefs(lookup'[idx+1..]);
+
+      forall i | P.ValidLayerIndex(lookup'[idx..], i) && i < |lookup'[idx..]| - 1 
+      ensures P.LookupFollowsChildRefAtLayer(lookup'[idx..], i)
+      ensures P.LookupFollowsChildEdgeAtLayer(lookup'[idx..], i)
+      {
+        if i == 0 {
+          assert lookup'[idx..][i] == lookup'[idx];
+          assert P.LookupFollowsChildRefAtLayer(lookup', idx);
+          assert P.LookupFollowsChildRefAtLayer(lookup, idx);
+          assert P.LookupFollowsChildRefAtLayer(lookup'[idx..], i);
+
+          var prefix1 := if idx == 0 then None else tt[idx-1];
+          var prefix2 := Translate(pivots, edges, lookup[idx].currentKey);
+          var prefix3 := Translate(pivots, edges, lookup'[idx].currentKey);
+          assert prefix2 == prefix3;
+
+          InRangeImpliesSameRoute(start, key, end, lookup, tt, lookup', idx+1);
+          assert tt[idx] == ComposePrefixSet(prefix1, prefix2) by {
+            P.reveal_LookupTranslationTable();
+          }
+          assert key == ApplyPrefixSet(prefix1, lookup'[idx].currentKey) by {
+            reveal_IsPrefix();
+          }
+          ComposePrefixSetCorrect(prefix1, prefix2, tt[idx], key, 
+              lookup'[idx].currentKey, lookup'[idx+1].currentKey);
+          assert P.LookupFollowsChildEdgeAtLayer(lookup', idx);
+        } else {
+          assert lookup'[idx..][i] == lookup'[idx+1..][i-1];
+          assert P.LookupFollowsChildRefAtLayer(lookup'[idx+1..], i-1);
+          assert P.LookupFollowsChildRefAtLayer(lookup'[idx..], i);
+          assert P.LookupFollowsChildEdgeAtLayer(lookup'[idx+1..], i-1);
+          assert P.LookupFollowsChildEdgeAtLayer(lookup'[idx..], i);
+        }
+      }
+    }
+  }
+
+  lemma GenerateLookupWellMarshalled(start: MS.UI.RangeStart, key: Key, end: MS.UI.RangeEnd,
+    lookup: P.Lookup, lookup': P.Lookup, tt: TranslationTable, idx: int)
+  requires MS.InRange(start, key, end)
+  requires P.ValidLayerIndex(lookup, idx)
+  requires P.LookupVisitsWFNodes(lookup)
+  requires P.LookupBoundedKey(lookup)
+  requires lookup[0].currentKey == if start.NegativeInf? then [] else start.key
+  requires P.ValidTranslationTable(lookup, tt, 0)
+  requires lookup' == GenerateLookup(lookup, key, tt, 0)
+  requires
+    var lookupUpperBound := P.LookupUpperBound(lookup, tt);
+    && (lookupUpperBound.Some? ==> !MS.UpperBound(lookupUpperBound.value, end))
+  requires P.LookupBoundedKey(lookup')
+  ensures P.LookupVisitsWellMarshalledBuckets(lookup) ==> 
+      P.LookupVisitsWellMarshalledBuckets(lookup'[idx..])
+  decreases |lookup'| - idx
+  {
+    InRangeImpliesSameRoute(start, key, end, lookup, tt, lookup', idx);
+    if idx < |lookup'| - 1 {
+      GenerateLookupWellMarshalled(start, key, end, lookup, lookup', tt, idx+1);
+    }
+  }
+
+  lemma WFGenerateLookup(start: MS.UI.RangeStart, key: Key, end: MS.UI.RangeEnd,
+    lookup: P.Lookup, lookup': P.Lookup, tt: TranslationTable)
+  requires MS.InRange(start, key, end)
+  requires
+    var startKey := if start.NegativeInf? then [] else start.key;
+    && P.WFLookupForKey(lookup, startKey)
+  requires tt == P.LookupTranslationTable(lookup, 0, None)
+  requires lookup' == GenerateLookup(lookup, key, tt, 0)
+  requires
+    var lookupUpperBound := P.LookupUpperBound(lookup, tt);
+    && (lookupUpperBound.Some? ==> !MS.UpperBound(lookupUpperBound.value, end))
+  ensures P.WFLookupForKey(lookup', key)
+  ensures P.LookupVisitsWellMarshalledBuckets(lookup) ==> 
+      P.LookupVisitsWellMarshalledBuckets(lookup')
+  {
+    WFGenerateLookupIter(start, key, end, lookup, lookup', tt, 0);
+    GenerateLookupWellMarshalled(start, key, end, lookup, lookup', tt, 0);
   }
  
   function InterpretBucketStack(buckets: seq<Bucket>, key: Key) : Message
@@ -506,62 +703,109 @@ module PivotBetreeSpecRefinement {
     }
   }
 
-  lemma InterpretBucketStackEqInterpretLookupIter(
-      start: MS.UI.RangeStart, end: MS.UI.RangeEnd, startKey: Key,
-      buckets: seq<Bucket>, lookup: P.Lookup, key: Key,
-      j: int)
-  requires startKey == if start.NegativeInf? then [] else start.key;
-  requires P.LookupVisitsWFNodes(lookup)
-  requires P.LookupBoundedKey(startKey, lookup)
+  lemma SuccBucketAtLayerPreservesLookup(lookup: P.Lookup, lookup': P.Lookup,
+    buckets: seq<Bucket>, buckets': seq<Bucket>, tt: TranslationTable, key: Key, idx: int)
+  requires 1 <= idx
   requires |lookup| == |buckets|
-  requires (forall i | 0 <= i < |lookup| :: buckets[i] == lookup[i].node.buckets[Route(lookup[i].node.pivotTable, startKey)])
-  requires MS.InRange(start, key, end)
-  requires
-    var lookupUpperBound := P.LookupUpperBound(lookup, startKey);
-    && P.WFLookupForKey(lookup, startKey)
-    && (lookupUpperBound.Some? ==> !MS.UpperBound(lookupUpperBound.value, end))
-  requires 0 <= j <= |lookup|
-  requires P.LookupBoundedKey(key, lookup)
-  requires P.LookupVisitsWellMarshalledBuckets(lookup, key)
-  requires BucketListWellMarshalled(buckets)
-  ensures InterpretBucketStack(buckets[..j], key)
-       == P.InterpretLookup(lookup[..j], key)
+  requires |lookup| == |lookup'|
+  requires |buckets| == |buckets'|
+  requires P.SuccBucketAtLayer.requires(buckets, tt, idx)
+  requires buckets'[idx] == P.SuccBucketAtLayer(buckets, tt, idx)
+  requires BucketWellMarshalled(buckets[idx])
+  requires lookup[idx].readOp == lookup'[idx].readOp
+  requires P.G.Keyspace.lte(lookup[idx].currentKey, lookup'[idx].currentKey)
+  requires P.WFNode(lookup[idx].readOp.node)
+  requires BoundedKey(lookup[idx].readOp.node.pivotTable, lookup[idx].currentKey)
+  requires BoundedKey(lookup'[idx].readOp.node.pivotTable, lookup'[idx].currentKey)
+  requires Route(lookup[idx].readOp.node.pivotTable, lookup[idx].currentKey)
+        == Route(lookup'[idx].readOp.node.pivotTable, lookup'[idx].currentKey)
+  requires buckets[idx] == lookup[idx].readOp.node.buckets[
+      Route(lookup[idx].readOp.node.pivotTable, lookup[idx].currentKey)]
+  requires tt[idx-1].Some? ==> IsPrefix(tt[idx-1].value.prefix, lookup'[idx].currentKey)
+  requires key == ApplyPrefixSet(tt[idx-1], lookup'[idx].currentKey)
+  ensures P.NodeLookup(lookup'[idx].readOp.node, lookup'[idx].currentKey)
+          == BucketGet(buckets'[idx].as_map(), key)
   {
-    if j == 0 {
+    var r := Route(lookup'[idx].readOp.node.pivotTable, lookup'[idx].currentKey);
+    if tt[idx-1].None? {
+      assert lookup'[idx].readOp.node.buckets[r] == buckets'[idx];
     } else {
-      InRangeImpliesSameRoute(start, key, end, lookup, j-1);
-      //var layer := lookup[j-1]
-      //assert Route(layer.node.pivotTable, key) == Route(layer.node.pivotTable, startKey);
-
-      InterpretBucketStackEqInterpretLookupIter(start, end, startKey,
-          buckets, lookup, key, j-1);
-      assert DropLast(buckets[..j]) == buckets[..j-1];
-      assert DropLast(lookup[..j]) == lookup[..j-1];
+      TranslateBucketSameMessage(buckets[idx], buckets'[idx], tt[idx-1].value.prefix,
+        tt[idx-1].value.newPrefix, lookup'[idx].currentKey, key);
     }
   }
 
-  lemma InterpretBucketStackEqInterpretLookup(
-      start: MS.UI.RangeStart, end: MS.UI.RangeEnd, startKey: Key,
-      buckets: seq<Bucket>, lookup: P.Lookup, key: Key)
-  requires startKey == if start.NegativeInf? then [] else start.key;
-  requires P.LookupVisitsWFNodes(lookup)
-  requires P.LookupBoundedKey(startKey, lookup)
-  requires |lookup| == |buckets|
-  requires (forall i | 0 <= i < |lookup| :: buckets[i] == lookup[i].node.buckets[Route(lookup[i].node.pivotTable, startKey)])
+  lemma InterpretBucketStackEqInterpretLookupIter(start: MS.UI.RangeStart, key: Key,
+    end: MS.UI.RangeEnd, lookup: P.Lookup, buckets: seq<Bucket>, lookup': P.Lookup,
+    buckets': seq<Bucket>, tt: TranslationTable, idx: int)
+  requires 1 <= idx <= |lookup| == |buckets|
   requires MS.InRange(start, key, end)
+  requires P.LookupVisitsWFNodes(lookup)
+  requires P.LookupBoundedKey(lookup)
+  requires lookup[0].currentKey == if start.NegativeInf? then [] else start.key
+  requires P.ValidTranslationTable(lookup, tt, 0)
+  requires lookup' == GenerateLookup(lookup, key, tt, 0)
+  requires P.LookupVisitsWFNodes(lookup')
+  requires P.LookupBoundedKey(lookup')
   requires
-    var lookupUpperBound := P.LookupUpperBound(lookup, startKey);
-    && P.WFLookupForKey(lookup, startKey)
+    var lookupUpperBound := P.LookupUpperBound(lookup, tt);
     && (lookupUpperBound.Some? ==> !MS.UpperBound(lookupUpperBound.value, end))
-  requires P.LookupBoundedKey(key, lookup)
-  requires P.LookupVisitsWellMarshalledBuckets(lookup, key)
+  requires forall i | 0 <= i < |lookup| :: buckets[i] 
+    == lookup[i].readOp.node.buckets[Route(lookup[i].readOp.node.pivotTable, lookup[i].currentKey)]
   requires BucketListWellMarshalled(buckets)
-  ensures InterpretBucketStack(buckets, key)
-       == P.InterpretLookup(lookup, key)
+  requires buckets' == P.TranslateSuccBuckets(buckets, tt, 0)
+  ensures InterpretBucketStack(buckets'[..idx], key)
+       == P.InterpretLookup(lookup'[..idx])
   {
-    InterpretBucketStackEqInterpretLookupIter(start, end, startKey, buckets, lookup, key, |lookup|);
-    assert buckets[..|buckets|] == buckets;
-    assert lookup[..|buckets|] == lookup;
+    assert |buckets| == |buckets'|;
+    assert |lookup| == |lookup'|;
+
+    InRangeImpliesSameRoute(start, key, end, lookup, tt, lookup', idx-1);
+
+    if idx == 1 {
+      assert key == lookup'[0].currentKey;
+      assert InterpretBucketStack(buckets'[..idx], key) == P.InterpretLookup(lookup'[..idx]);
+    } else {
+      assert key == ApplyPrefixSet(tt[idx-2], lookup'[idx-1].currentKey) by {
+        reveal_IsPrefix();
+      }
+      SuccBucketAtLayerPreservesLookup(lookup, lookup', buckets, buckets', tt, key, idx-1);
+      assert P.NodeLookup(lookup'[idx-1].readOp.node, lookup'[idx-1].currentKey) == BucketGet(buckets'[idx-1].as_map(), key);
+
+      assert DropLast(buckets'[..idx]) == buckets'[..idx-1];
+      assert DropLast(lookup'[..idx]) == lookup'[..idx-1];
+
+      InterpretBucketStackEqInterpretLookupIter(start, key, end, lookup, buckets, lookup', buckets', tt, idx-1);
+      // assert InterpretBucketStack(buckets'[..idx-1], key) == P.InterpretLookup(lookup'[..idx-1]);
+      assert InterpretBucketStack(buckets'[..idx], key) == P.InterpretLookup(lookup'[..idx]);
+    }
+  }
+
+  lemma InterpretBucketStackEqInterpretLookup(start: MS.UI.RangeStart, key: Key,
+    end: MS.UI.RangeEnd, lookup: P.Lookup, buckets: seq<Bucket>, lookup': P.Lookup,
+    buckets': seq<Bucket>, tt: TranslationTable)
+  requires MS.InRange(start, key, end)
+  requires 0 < |lookup| == |buckets|
+  requires P.LookupVisitsWFNodes(lookup)
+  requires P.LookupBoundedKey(lookup)
+  requires lookup[0].currentKey == if start.NegativeInf? then [] else start.key
+  requires P.ValidTranslationTable(lookup, tt, 0)
+  requires lookup' == GenerateLookup(lookup, key, tt, 0)
+  requires P.LookupVisitsWFNodes(lookup')
+  requires P.LookupBoundedKey(lookup')
+  requires
+    var lookupUpperBound := P.LookupUpperBound(lookup, tt);
+    && (lookupUpperBound.Some? ==> !MS.UpperBound(lookupUpperBound.value, end))
+  requires BucketListWellMarshalled(buckets)
+  requires forall i | 0 <= i < |lookup| :: buckets[i] 
+    == lookup[i].readOp.node.buckets[Route(lookup[i].readOp.node.pivotTable, lookup[i].currentKey)]
+  requires buckets' == P.TranslateSuccBuckets(buckets, tt, 0)
+  ensures InterpretBucketStack(buckets', key)
+       == P.InterpretLookup(lookup')
+  {
+    InterpretBucketStackEqInterpretLookupIter(start, key, end, lookup, buckets, lookup', buckets', tt, |buckets|);
+    assert buckets'[..|buckets'|] == buckets';
+    assert lookup'[..|buckets'|] == lookup';
   }
 
   lemma SuccQueryProperties(results: seq<UI.SuccResult>, buckets: seq<Bucket>,
@@ -624,38 +868,51 @@ module PivotBetreeSpecRefinement {
   {
     var q := ISuccQuery(sq);
     var startKey := if sq.start.NegativeInf? then [] else sq.start.key;
-
-    SuccQueryProperties(sq.results, sq.buckets, sq.start, sq.end);
+    var translatedbuckets := P.TranslateSuccBuckets(sq.buckets, sq.translations, 0);
+    SuccQueryProperties(sq.results, translatedbuckets, sq.start, sq.end);
 
     forall i | 0 <= i < |q.results|
-    ensures B.LookupKeyValue(q.lookup, q.results[i].key, q.results[i].value)
+    ensures (exists lookup :: B.SamePathWithKeyValue(q.lookup, lookup, q.results[i].key, q.results[i].value))
     {
-      InRangeImpliesValidLookup(sq.start, sq.results[i].key, sq.end, sq.lookup);
+      var lookup' := GenerateLookup(sq.lookup, sq.results[i].key, sq.translations, 0);
+      WFGenerateLookup(sq.start, sq.results[i].key, sq.end, sq.lookup, lookup', sq.translations);
+      SameILayersReadOp(sq.lookup, lookup');
 
-      RefinesLookup(sq.lookup, sq.results[i].key);
-      RefinesInterpretLookupAccountingForLeaf(sq.lookup, sq.results[i].key, sq.results[i].value);
+      RefinesLookup(lookup', sq.results[i].key);
+      RefinesInterpretLookupAccountingForLeaf(lookup', sq.results[i].key, sq.results[i].value);
 
-      InterpretBucketStackEqInterpretLookup(sq.start, sq.end, startKey, sq.buckets, sq.lookup, sq.results[i].key);
+      InterpretBucketStackEqInterpretLookup(sq.start, sq.results[i].key, sq.end, sq.lookup, sq.buckets, lookup', translatedbuckets, sq.translations);
+      assert B.InterpretLookup(ILayers(lookup')) == P.InterpretLookup(lookup');
+      assert B.SamePathWithKeyValue(q.lookup, ILayers(lookup'), q.results[i].key, q.results[i].value);
     }
+
+    assert (forall r | r in q.results :: (exists lookup :: B.SamePathWithKeyValue(q.lookup, lookup, r.key, r.value)));
 
     forall key | MS.InRange(q.start, key, q.end)
         && (forall i | 0 <= i < |q.results| :: q.results[i].key != key)
-    ensures B.LookupKeyValue(q.lookup, key, MS.EmptyValue())
+    ensures (exists lookup :: B.SamePathWithKeyValue(q.lookup, lookup, key, MS.EmptyValue()))
     {
-      InRangeImpliesValidLookup(sq.start, key, sq.end, sq.lookup);
+      var lookup' := GenerateLookup(sq.lookup, key, sq.translations, 0);
+      WFGenerateLookup(sq.start, key, sq.end, sq.lookup, lookup', sq.translations);
+      SameILayersReadOp(sq.lookup, lookup');
 
-      RefinesLookup(sq.lookup, key);
-      RefinesInterpretLookupAccountingForLeaf(sq.lookup, key, MS.EmptyValue());
-      //assert P.BufferDefinesEmptyValue(P.InterpretLookup(sq.lookup, key));
-      //assert P.InterpretLookupAccountingForLeaf(sq.lookup, key) == M.DefineDefault();
-
-      //assert M.DefaultValue() == MS.EmptyValue();
+      RefinesLookup(lookup', key);
+      RefinesInterpretLookupAccountingForLeaf(lookup', key, MS.EmptyValue());
 
       /*assert B.InterpretLookup(IReadOps(sq.lookup), key).value
           == P.InterpretLookupAccountingForLeaf(sq.lookup, key).value
           == MS.EmptyValue();*/
 
-      InterpretBucketStackEqInterpretLookup(sq.start, sq.end, startKey, sq.buckets, sq.lookup, key);
+      assert P.LookupVisitsWellMarshalledBuckets(lookup');
+      assert B.InterpretLookup(ILayers(lookup')) == P.InterpretLookupAccountingForLeaf(lookup');
+
+      InterpretBucketStackEqInterpretLookup(sq.start, key, sq.end, sq.lookup, sq.buckets, lookup', translatedbuckets, sq.translations);
+
+      assert InterpretBucketStack(translatedbuckets, key) == P.InterpretLookup(lookup');
+      assert P.BufferDefinesEmptyValue(P.InterpretLookup(lookup'));
+
+      assert B.LookupKeyValue(ILayers(lookup'), key, MS.EmptyValue());
+      assert B.SamePathWithKeyValue(q.lookup, ILayers(lookup'), key, MS.EmptyValue());
     }
   }
 
@@ -664,6 +921,135 @@ module PivotBetreeSpecRefinement {
   requires ReadOpsBucketsWellMarshalled(P.InsertionReads(ins))
   ensures B.ValidInsertion(IInsertion(ins))
   {
+  }
+
+  lemma RefinesValidFlushNewParent(flush: P.NodeFlush)
+  requires P.ValidFlush(flush)
+  requires P.InvNode(flush.parent)
+  requires P.InvNode(flush.child)
+  requires (forall key | key in IFlush(flush).flushedkeys :: key in IFlush(flush).parent.children)
+  ensures B.ValidFlushNewParent(IFlush(flush))
+  {
+    var f := IFlush(flush);
+
+    var child' := P.RestrictAndTranslateChild(flush.parent, flush.child, flush.slot_idx);
+    PivotBetreeSpecWFNodes.RestrictAndTranslateWFProperWellMarshalled(flush.parent, flush.child, flush.slot_idx);
+    assert child'.pivotTable[0] == flush.parent.pivotTable[flush.slot_idx];
+    assert Last(child'.pivotTable) == flush.parent.pivotTable[flush.slot_idx+1];
+
+    var flushedKeys := BucketFlushModel.partialFlushCorrect(
+      flush.parent.buckets[flush.slot_idx], child'.pivotTable, child'.buckets);
+    reveal_BucketIntersect();
+    reveal_BucketComplement();
+  }
+
+  lemma ValidFlushNewChildChildren(flush: P.NodeFlush, f: B.NodeFlush)
+  requires P.ValidFlush(flush)
+  requires P.InvNode(flush.parent)
+  requires P.InvNode(flush.child)
+  requires P.InvNode(flush.newchild)
+  requires f == IFlush(flush)
+  requires (forall key | key in f.movedkeys :: key in f.parent.children)
+  ensures IChildren(flush.newchild) ==
+     (imap k | k in f.movedkeys && f.parent.children[k].edgeKey in f.child.children :: 
+        f.child.children[f.parent.children[k].edgeKey])
+  {
+    if flush.child.children.Some? {
+      var child' := P.RestrictAndTranslateChild(flush.parent, flush.child, flush.slot_idx);
+      assert child'.pivotTable[0] == flush.parent.pivotTable[flush.slot_idx];
+      assert Last(child'.pivotTable) == flush.parent.pivotTable[flush.slot_idx+1];
+
+      forall k | k !in f.movedkeys || f.parent.children[k].edgeKey !in f.child.children
+      ensures k !in IChildren(child')
+      {
+        if k !in f.movedkeys {
+          assert k !in IChildren(child');
+       } else if f.parent.children[k].edgeKey !in f.child.children {
+          RestrictAndTranslateKeyConsistency(flush.parent, flush.child, child', flush.slot_idx, k);
+          assert k !in IChildren(child');
+        }
+      }
+
+      forall k | k in f.movedkeys && f.parent.children[k].edgeKey in f.child.children
+      ensures k in IChildren(child')
+      ensures IChildren(child')[k] == f.child.children[f.parent.children[k].edgeKey]
+      {
+        RestrictAndTranslateKeyConsistency(flush.parent, flush.child, child', flush.slot_idx, k);
+        assert k in IChildren(child');
+      }
+    }
+  }
+
+  lemma RefinesValidFlushNewChild(flush: P.NodeFlush)
+  requires P.ValidFlush(flush)
+  requires P.InvNode(flush.parent)
+  requires P.InvNode(flush.child)
+  requires P.InvNode(flush.newchild)
+  requires (forall key | key in IFlush(flush).movedkeys :: key in IFlush(flush).parent.children)
+  ensures B.ValidFlushNewChild(IFlush(flush))
+  {
+    var f := IFlush(flush);
+
+    var child' := P.RestrictAndTranslateChild(flush.parent, flush.child, flush.slot_idx);
+    PivotBetreeSpecWFNodes.RestrictAndTranslateWFProperWellMarshalled(flush.parent, flush.child, flush.slot_idx);
+    assert child'.pivotTable[0] == flush.parent.pivotTable[flush.slot_idx];
+    assert Last(child'.pivotTable) == flush.parent.pivotTable[flush.slot_idx+1];
+
+    ValidFlushNewChildChildren(flush, f);
+
+    var tmpbuffer := imap k | k in f.movedkeys :: f.child.buffer[f.parent.children[k].edgeKey];
+    var newbuffer := imap k | k in f.movedkeys :: if k in f.flushedkeys then Merge(f.parent.buffer[k], tmpbuffer[k]) else tmpbuffer[k];
+    
+    forall k | k in f.movedkeys 
+    ensures IBuffer(child')[k] == tmpbuffer[k]
+    {
+      RestrictAndTranslateKeyConsistency(flush.parent, flush.child, child', flush.slot_idx, k);
+    }
+
+    var flushedKeys := BucketFlushModel.partialFlushCorrect(
+      flush.parent.buckets[flush.slot_idx], child'.pivotTable, child'.buckets);
+
+    reveal_BucketComplement();
+    reveal_BucketIntersect();
+
+    var isec := BucketIntersect(flush.parent.buckets[flush.slot_idx].as_map(), flushedKeys);
+
+    forall k | k in f.movedkeys
+    ensures IMapsAgreeOnKey(f.newchild.buffer, newbuffer, k) 
+    {
+      AddMessagesToNodeResult(child', isec, flush.newchild, k);
+      if k in isec {
+        if (flush.newchild.children.None?) {
+           MergeIsAssociative(BucketGet(isec, k), IBuffer(child')[k], DefineDefault());
+        }
+      } else {
+        assert newbuffer[k] == IBuffer(child')[k];
+        assert k !in f.flushedkeys; // observe
+        assert IBuffer(child')[k] == f.newchild.buffer[k];
+      }
+    }
+  }
+
+  lemma AddMessagesToNodeResult(node: PNode, bucket: BucketMap, node': PNode, key: Key)
+  requires WFPivots(node.pivotTable)
+  requires P.WFNode(node')
+  requires WFBucketListProper(node.buckets, node.pivotTable)
+  requires BucketListWellMarshalled(node.buckets)
+  requires WFBucketListProper(node'.buckets, node'.pivotTable);
+  requires BoundedKey(node.pivotTable, key)
+  requires BoundedKey(node'.pivotTable, key)
+  requires node'.pivotTable == node.pivotTable
+  requires node'.children == node.children
+  requires |node'.buckets| == |node.buckets|
+  requires forall i | 0 <= i < |node.buckets| ::
+      node'.buckets[i].as_map() == BucketListItemFlush(bucket, node.buckets[i].as_map(), node.pivotTable, i)
+  ensures WFBucketListProper(node'.buckets, node'.pivotTable);
+  ensures key !in bucket ==> IBuffer(node')[key] == IBuffer(node)[key]
+  ensures key in bucket ==> IBuffer(node')[key] == Merge(bucket[key], IBuffer(node)[key])
+  {
+    var i := Route(node.pivotTable, key);
+    assert node'.buckets[i].as_map() == 
+        BucketListItemFlush(bucket, node.buckets[i].as_map(), node.pivotTable, i);
   }
 
   lemma {:timeLimitMultiplier 4} RefinesValidFlush(flush: P.NodeFlush)
@@ -678,42 +1064,20 @@ module PivotBetreeSpecRefinement {
     assert P.InvNode(P.FlushReads(flush)[0].node);
     assert P.InvNode(P.FlushReads(flush)[1].node);
 
-    forall key | key in flush.parent.buckets[flush.slotIndex].as_map().Keys
+    forall key | key in flush.parent.buckets[flush.slot_idx].as_map().Keys
     ensures BoundedKey(flush.parent.pivotTable, key)
-    ensures Route(flush.parent.pivotTable, key) == flush.slotIndex
+    ensures Route(flush.parent.pivotTable, key) == flush.slot_idx
     {
       assert WFBucketAt(
-        flush.parent.buckets[flush.slotIndex],
+        flush.parent.buckets[flush.slot_idx],
         flush.parent.pivotTable,
-        flush.slotIndex);
+        flush.slot_idx);
       PivotBetreeSpecWFNodes.bucket_keys_in_seq(
-          flush.parent.buckets[flush.slotIndex]);
+          flush.parent.buckets[flush.slot_idx]);
     }
 
-    assert (forall key | key in f.movedKeys :: IMapsTo(f.parent.children, key, f.childref));
-    assert f.newparent.children == (imap k | k in f.parent.children :: (if k in f.movedKeys then f.newchildref else f.parent.children[k]));
-    assert f.newchild.children == f.child.children;
-
-    var flushedKeys := BucketFlushModel.partialFlushCorrect(
-      flush.parent.buckets[flush.slotIndex], flush.child.pivotTable, flush.child.buckets);
-
-    reveal_BucketIntersect();
-    reveal_BucketComplement();
-
-    assert f.newparent.buffer == 
-      (imap k : Key :: (if k in f.flushedKeys then IdentityMessage() else f.parent.buffer[k])); // observe
-
-    var isec := BucketIntersect(flush.parent.buckets[flush.slotIndex].as_map(), flushedKeys);
-    forall k: Key | BoundedKey(flush.child.pivotTable, k)
-    ensures f.newchild.buffer[k] == (if k in f.flushedKeys then Merge(f.parent.buffer[k], f.child.buffer[k]) else f.child.buffer[k])
-    {
-      AddMessagesToNodeResult(flush.child, isec, flush.newchild, k);
-      if (k in f.flushedKeys) {
-        if (flush.newchild.children.None?) {
-           MergeIsAssociative(BucketGet(isec, k), P.NodeLookup(flush.child, k), DefineDefault());
-        }
-      }
-    }
+    RefinesValidFlushNewParent(flush);
+    RefinesValidFlushNewChild(flush);
   }
 
   lemma RefinesValidGrow(growth: P.RootGrowth)
@@ -743,7 +1107,7 @@ module PivotBetreeSpecRefinement {
     assert Keyspace.lt(KeyToElement(key), node.pivotTable[i+1]);
     RouteIs(node.pivotTable, key, i);
     PivotBetreeSpecWFNodes.SplitMaps(node.buckets[cLeft], pivot);
-    //assert MapsAgreeOnKey(node.buckets[i].as_map(), node'.buckets[i].as_map(), key);
+    assert MapsAgreeOnKey(node.buckets[i].as_map(), node'.buckets[i].as_map(), key);
   }
 
   lemma CutoffNodeAndKeepRightAgree(node: PNode, node': PNode, pivot: Key, key: Key)
@@ -765,9 +1129,8 @@ module PivotBetreeSpecRefinement {
   }
 
   lemma CutoffNodeAgree(node: PNode, node': PNode, l: Key, r: Option<Key>, key: Key)
-  requires P.WFNode(node)
+  requires P.InvNode(node)
   requires P.WFNode(node')
-  requires BucketListWellMarshalled(node.buckets)
   requires P.ValidSplitKey(node, l, r)
   requires node' == P.CutoffNode(node, l, r)
   requires P.G.Keyspace.lte(l, key)
@@ -778,8 +1141,8 @@ module PivotBetreeSpecRefinement {
     P.reveal_CutoffNode();
     if (r.Some?) {
       var node1 := P.CutoffNodeAndKeepLeft(node, r.value);
-      PivotBetreeSpecWFNodes.BucketListWellMarshalledCutoffNodeAndKeepLeft(node, r.value);
       CutoffNodeAndKeepLeftAgree(node, node1, r.value, key);
+      PivotBetreeSpecWFNodes.KeepLeftWFProperWellMarshalled(node, r.value);
       CutoffNodeAndKeepRightAgree(node1, node', l, key);
     } else {
       CutoffNodeAndKeepRightAgree(node, node', l, key);
@@ -789,16 +1152,15 @@ module PivotBetreeSpecRefinement {
   lemma WriteFusedChildInTermsOfLeftAndRight(l: PNode, r: PNode, child: PNode, pivot: Key, num_children_left: int)
   requires P.WFNode(l)
   requires P.WFNode(r)
-  requires P.WFNode(child)
+  requires WFPivots(child.pivotTable)
+  requires WFEdges(child.edgeTable, child.pivotTable)
+  requires |child.buckets| == NumBuckets(child.pivotTable)
+  requires child.children.Some? ==> 0 <= num_children_left <= |child.children.value|
   requires 1 <= num_children_left < |child.buckets|
   requires l == P.SplitChildLeft(child, num_children_left)
   requires r == P.SplitChildRight(child, num_children_left)
   requires child.pivotTable[num_children_left].e == pivot
-  ensures child == P.G.Node(
-      concat3(l.pivotTable[..|l.pivotTable|-1], KeyToElement(pivot), r.pivotTable[1..]),
-      if l.children.Some? then Some(l.children.value + r.children.value) else None,
-      l.buckets + r.buckets
-    )
+  ensures child == P.FusedChild(l, r, pivot)
   {
     reveal_concat3();
     assert child.pivotTable == concat3(l.pivotTable[..|l.pivotTable|-1], KeyToElement(pivot), r.pivotTable[1..]);
@@ -814,32 +1176,33 @@ module PivotBetreeSpecRefinement {
   lemma MergedNodeAndLeftAgree(l: PNode, r: PNode, node: PNode, pivot: Key, key: Key)
   requires P.WFNode(l)
   requires P.WFNode(r)
-  requires P.WFNode(node)
+  requires WFPivots(node.pivotTable)
+  requires WFEdges(node.edgeTable, node.pivotTable)
+  requires NumBuckets(node.pivotTable) == |node.buckets|
+  requires (node.children.Some? ==> |node.buckets| == |node.children.value|)
   requires BoundedKey(l.pivotTable, key) && P.G.Keyspace.lt(key, pivot)
   requires l.children.Some? <==> r.children.Some?
-  requires node == P.G.Node(
-      concat3(l.pivotTable[..|l.pivotTable|-1], KeyToElement(pivot), r.pivotTable[1..]),
-      if l.children.Some? then Some(l.children.value + r.children.value) else None,
-      l.buckets + r.buckets
-    )
+  requires Last(l.pivotTable) == r.pivotTable[0] == KeyToElement(pivot)
+  requires node == P.FusedChild(l, r, pivot)
   ensures IBuffer(l)[key] == IBuffer(node)[key]
   ensures IMapsAgreeOnKey(IChildren(l), IChildren(node), key)
   {
     var i := Route(l.pivotTable, key);
     RouteIs(node.pivotTable, key, i);
+    WFConcatEdges(l.pivotTable, l.edgeTable, r.pivotTable, r.edgeTable, node.pivotTable);
   }
 
   lemma MergedNodeAndRightAgree(l: PNode, r: PNode, node: PNode, pivot: Key, key: Key)
   requires P.WFNode(l)
   requires P.WFNode(r)
-  requires P.WFNode(node)
+  requires WFPivots(node.pivotTable)
+  requires WFEdges(node.edgeTable, node.pivotTable)
+  requires NumBuckets(node.pivotTable) == |node.buckets|
+  requires (node.children.Some? ==> |node.buckets| == |node.children.value|)
   requires BoundedKey(r.pivotTable, key) && P.G.Keyspace.lte(pivot, key)
+  requires Last(l.pivotTable) == r.pivotTable[0] == KeyToElement(pivot)
   requires l.children.Some? <==> r.children.Some?
-  requires node == P.G.Node(
-      concat3(l.pivotTable[..|l.pivotTable|-1], KeyToElement(pivot), r.pivotTable[1..]),
-      if l.children.Some? then Some(l.children.value + r.children.value) else None,
-      l.buckets + r.buckets
-    )
+  requires node == P.FusedChild(l, r, pivot)
   ensures IBuffer(r)[key] == IBuffer(node)[key]
   ensures IMapsAgreeOnKey(IChildren(r), IChildren(node), key)
   {
@@ -849,46 +1212,30 @@ module PivotBetreeSpecRefinement {
     }
     assert node.pivotTable[i+|l.buckets|+1] == r.pivotTable[i+1];
     RouteIs(node.pivotTable, key, i + |l.buckets|);
-  }
-
-  lemma ValidLeftChildHasGoodPivots(f: P.NodeFusion)
-  requires P.ValidSplit(f)
-  ensures Keyspace.lte(f.split_parent.pivotTable[f.slot_idx], f.left_child.pivotTable[0])
-  ensures Keyspace.lte(Last(f.left_child.pivotTable), f.split_parent.pivotTable[f.slot_idx+1])
-  {
-  }
-
-  lemma ValidRightChildHasGoodPivots(f: P.NodeFusion)
-  requires P.ValidSplit(f)
-  ensures Keyspace.lte(f.split_parent.pivotTable[f.slot_idx+1], f.right_child.pivotTable[0])
-  ensures Keyspace.lte(Last(f.right_child.pivotTable), f.split_parent.pivotTable[f.slot_idx+2])
-  {
-  }
-
-  lemma ValidMergeChildHasGoodPivots(f: P.NodeFusion)
-  requires P.ValidMerge(f)
-  ensures Keyspace.lte(f.fused_parent.pivotTable[f.slot_idx], f.fused_child.pivotTable[0])
-  ensures Keyspace.lte(Last(f.fused_child.pivotTable), f.fused_parent.pivotTable[f.slot_idx+1])
-  {
+    WFConcatEdges(l.pivotTable, l.edgeTable, r.pivotTable, r.edgeTable, node.pivotTable);
   }
 
   lemma SplitMergeBuffersChildrenEq(node: PNode, node': PNode, idx: int)
   requires P.WFNode(node)
   requires P.WFNode(node')
-  requires BucketListWellMarshalled(node.buckets)
-  requires |node'.buckets| == |node.buckets| + 1
-  requires 0 <= idx < |node.buckets|
-  requires forall i | 0 <= i < idx :: node.buckets[i] == node'.buckets[i]
-  requires node'.buckets[idx] == SplitBucketLeft(node.buckets[idx], GetKey(node'.pivotTable, idx+1))
-  requires node'.buckets[idx+1] == SplitBucketRight(node.buckets[idx], GetKey(node'.pivotTable, idx+1))
-  requires forall i | idx + 2 <= i < |node'.buckets| :: node'.buckets[i] == node.buckets[i-1]
-  requires forall i | 0 <= i <= idx :: node.pivotTable[i] == node'.pivotTable[i]
-  requires forall i | idx+1 < i < |node'.pivotTable| :: node'.pivotTable[i] == node.pivotTable[i-1]
   requires node.children.Some?
   requires node'.children.Some?
-  requires forall i | 0 <= i < idx :: node.children.value[i] == node'.children.value[i]
-  requires forall i | idx + 2 <= i < |node'.buckets| :: node'.children.value[i] == node.children.value[i-1]
-  requires forall key :: BoundedKey(node.pivotTable, key) <==> BoundedKey(node'.pivotTable, key) // TODO: revisit
+  requires BucketListWellMarshalled(node.buckets)
+  requires 0 <= idx < |node.buckets|
+  requires |node'.buckets| == |node.buckets| + 1
+  requires node'.buckets[idx] == SplitBucketLeft(node.buckets[idx], GetKey(node'.pivotTable, idx+1))
+  requires node'.buckets[idx+1] == SplitBucketRight(node.buckets[idx], GetKey(node'.pivotTable, idx+1))
+  requires forall i | 0 <= i < idx :: 
+    && node.buckets[i] == node'.buckets[i]
+    && node.edgeTable[i] == node'.edgeTable[i]
+    && node.children.value[i] == node'.children.value[i]
+  requires forall i | idx + 2 <= i < |node'.buckets| :: 
+    && node.buckets[i-1] == node'.buckets[i]
+    && node.edgeTable[i-1] == node'.edgeTable[i]
+    && node.children.value[i-1] == node'.children.value[i]
+  requires forall i | 0 <= i <= idx :: node.pivotTable[i] == node'.pivotTable[i]
+  requires forall i | idx+1 < i < |node'.pivotTable| :: node'.pivotTable[i] == node.pivotTable[i-1]
+  requires forall key :: BoundedKey(node.pivotTable, key) <==> BoundedKey(node'.pivotTable, key)
   ensures IBuffer(node) == IBuffer(node')
   ensures forall key:Key | key !in PivotTableBucketKeySet(node.pivotTable, idx) && BoundedKey(node.pivotTable, key) ::
       IChildren(node)[key] == IChildren(node')[key]
@@ -924,66 +1271,230 @@ module PivotBetreeSpecRefinement {
     }
   }
 
-  lemma MergeRouteNewChild(f: P.NodeFusion, r: B.Redirect, childref: Reference, ref: Reference) returns (key: Key)
-  requires P.ValidMerge(f)
-  requires P.InvNode(f.split_parent)
-  requires P.InvNode(f.left_child)
-  requires P.InvNode(f.right_child)
-  requires r == IMerge(f)
-  requires childref in r.new_children
-  requires ref in r.new_children[childref].children.Values
-  ensures IMapsTo(r.new_parent.children, key, childref)
-        && IMapsTo(r.new_children[childref].children, key, ref)
-        && key in r.keys
-        && key in r.old_parent.children
+  lemma RestrictAndTranslateKeyConsistency(parent: PNode, child: PNode, child': PNode, slot: int, key: Key)
+  requires P.InvNode(parent)
+  requires P.InvNode(child)
+  requires 0 <= slot < NumBuckets(parent.pivotTable)
+  requires ParentKeysInChildRange(parent.pivotTable, parent.edgeTable, child.pivotTable, slot)
+  requires BoundedKey(parent.pivotTable, key) && Route(parent.pivotTable, key) == slot
+  requires child' == P.RestrictAndTranslateChild(parent, child, slot)
+  ensures BoundedKey(child'.pivotTable, key)
+  ensures var edgekey := TranslateKey(parent.pivotTable, parent.edgeTable, key);
+    && IBuffer(child')[key] == IBuffer(child)[edgekey]
+    && (key in IChildren(child') <==> edgekey in IChildren(child))
+    && (key in IChildren(child') ==> IChildren(child')[key] == IChildren(child)[edgekey])
   {
-    PivotBetreeSpecWFNodes.ValidMergeWritesInvNodes(f);
-    assert childref == f.fused_childref;
-    var new_child := r.new_children[childref];
-    var k :| k in new_child.children && new_child.children[k] == ref;
-    var i := Route(f.fused_child.pivotTable, k);
-    
-    ValidMergeChildHasGoodPivots(f);
-    key := GetKeyInChildBucket(f.fused_parent.pivotTable, f.fused_child.pivotTable, f.slot_idx, i);
+    if parent.edgeTable[slot].None? {
+      var lbound := P.getlbound(parent, slot);
+      var ubound := P.getubound(parent, slot);
+
+      ContainsRangeImpliesBoundedKey(child.pivotTable, parent.pivotTable[slot], parent.pivotTable[slot+1]);
+      CutoffNodeAgree(child, child', lbound, ubound, key);
+    } else {
+      var (lbound, ubound) := TranslatePivotPair(parent.pivotTable, parent.edgeTable, slot);
+      var lboundkey : Key := lbound.e;
+      var uboundkey := if ubound.Element? then (var k: Key := ubound.e; Some(k)) else None;
+      var tmpchild := P.CutoffNode(child, lboundkey, uboundkey);
+
+      var parentprefix := PivotLcp(parent.pivotTable[slot], parent.pivotTable[slot+1]);
+      var childprefix := parent.edgeTable[slot].value;
+      var edgekey := TranslateKey(parent.pivotTable, parent.edgeTable, key);
+
+      TranslatePivotPairRangeProperty(parent.pivotTable[slot], parent.pivotTable[slot+1], parentprefix, childprefix);
+      CutoffNodeAgree(child, tmpchild, lboundkey, uboundkey, edgekey);
+      PivotBetreeSpecWFNodes.CutoffNodeWFProperWellMarshalled(child, lboundkey, uboundkey);
+
+      assert child'.pivotTable[0] == parent.pivotTable[slot];
+      assert Last(child'.pivotTable) == parent.pivotTable[slot+1]; // observe
+      TranslatePivotsSameRoute(tmpchild.pivotTable,child'.pivotTable, childprefix, parentprefix, edgekey, key);
+      TranslatePivotsEdgesPreserveTranslateKey(tmpchild.pivotTable, tmpchild.edgeTable, child'.pivotTable,
+        child'.edgeTable, childprefix, parentprefix, parent.pivotTable[slot+1], edgekey, key);
+      
+      var i := Route(tmpchild.pivotTable, edgekey);
+      TranslateBucketSameMessage(tmpchild.buckets[i], child'.buckets[i], childprefix, parentprefix, edgekey, key);
+    }
   }
 
-  lemma MergeChildrenConsistent(f: P.NodeFusion, r: B.Redirect, key: Key)
+  lemma MergeRefinesWFRedirect(f: P.NodeFusion)
   requires P.ValidMerge(f)
   requires P.InvNode(f.split_parent)
   requires P.InvNode(f.left_child)
   requires P.InvNode(f.right_child)
-  requires P.InvNode(f.fused_parent);
-  requires P.InvNode(f.fused_child);
-  requires r == IMerge(f)
-  requires key in r.keys * r.old_parent.children.Keys
-  ensures r.old_parent.children[key] in r.old_children
-  ensures IMapsAgreeOnKey(
-      r.new_children[r.new_parent.children[key]].buffer,
-      r.old_children[r.old_parent.children[key]].buffer, key)
-  ensures IMapsAgreeOnKey(
-      r.new_children[r.new_parent.children[key]].children,
-      r.old_children[r.old_parent.children[key]].children, key)
+  requires P.InvNode(f.fused_parent)
+  requires P.InvNode(f.fused_child)
+  ensures B.WFRedirect(IMerge(f))
   {
-    var lb := P.getlbound(f.split_parent, f.slot_idx);
-    var ub := P.getubound(f.split_parent, f.slot_idx+1);
+    var r := IMerge(f);
+    var old_parent_children_ref := imap k | k in r.old_parent.children :: r.old_parent.children[k].ref;
 
-    var left := P.CutoffNode(f.left_child, lb , Some(f.pivot));
-    var right := P.CutoffNode(f.right_child, f.pivot, ub);
+    forall ref | ref in r.old_childrefs
+    ensures ref in IMapRestrict(old_parent_children_ref, r.keys).Values
+    {
+      assert ref == f.left_childref || ref == f.right_childref;
+      if (ref == f.left_childref) {
+        var key := GetKeyInBucket(f.split_parent.pivotTable, f.slot_idx);
+        RouteIs(f.fused_parent.pivotTable, key, f.slot_idx);
+        assert key in r.keys;
+        assert key in IMapRestrict(r.old_parent.children, r.keys);
+        assert IMapRestrict(old_parent_children_ref, r.keys)[key] == ref;
+        assert ref in IMapRestrict(old_parent_children_ref, r.keys).Values;
+      } else {
+        var key := GetKeyInBucket(f.split_parent.pivotTable, f.slot_idx + 1);
+        RouteIs(f.fused_parent.pivotTable, key, f.slot_idx);
+        assert key in r.keys;
+        assert key in IMapRestrict(r.old_parent.children, r.keys);
+        assert IMapRestrict(old_parent_children_ref, r.keys)[key] == ref;
+        assert ref in IMapRestrict(old_parent_children_ref, r.keys).Values;
+      }
+    }
 
-    if (P.G.Keyspace.lt(key, f.pivot)) {
-      RouteIs(f.split_parent.pivotTable, key, f.slot_idx);
-      assert r.old_parent.children[key] == f.left_childref;
-      assert r.old_children[r.old_parent.children[key]] == INode(f.left_child);
-      CutoffNodeAgree(f.left_child, left, lb, Some(f.pivot), key);
+    forall ref | ref in IMapRestrict(old_parent_children_ref, r.keys).Values
+    ensures ref in r.old_childrefs
+    {
+      // var key: Key :| IMapsTo(IMapRestrict(old_parent_children_ref, r.keys), key, ref);
+      // assert key in r.keys;
+      // if (P.G.Keyspace.lt(key, f.pivot)) {
+      //   RouteIs(f.split_parent.pivotTable, key, f.slot_idx);
+      //   assert ref == f.left_childref;
+      // } else {
+      //   assert f.split_parent.pivotTable[f.slot_idx + 2] == f.fused_parent.pivotTable[f.slot_idx + 1];
+      //   RouteIs(f.split_parent.pivotTable, key, f.slot_idx+1);
+      //   assert ref == f.right_childref;
+      // }
+    }
+
+    assert forall k | k in r.keys :: Keyspace.lt(KeyToElement(k), f.fused_parent.pivotTable[f.slot_idx+1]);
+    assert B.WFRedirect(r);
+  }
+
+  lemma MergeRefinesRedirectNewParent(f: P.NodeFusion)
+  requires P.ValidMerge(f)
+  requires P.InvNode(f.split_parent)
+  requires P.InvNode(f.left_child)
+  requires P.InvNode(f.right_child)
+  requires P.InvNode(f.fused_parent)
+  requires P.InvNode(f.fused_child)
+  requires B.WFRedirect(IMerge(f))
+  ensures B.ValidRedirectNewParent(IMerge(f))
+  {
+    reveal_MergeBucketsInList();
+    SplitOfMergeBucketsInList(f.split_parent.buckets, f.slot_idx, f.split_parent.pivotTable);
+    SplitMergeBuffersChildrenEq(f.fused_parent, f.split_parent, f.slot_idx);
+  }
+
+  lemma MergeRefinesRedirectNewChildren(f: P.NodeFusion)
+  requires P.ValidMerge(f)
+  requires P.InvNode(f.split_parent)
+  requires P.InvNode(f.left_child)
+  requires P.InvNode(f.right_child)
+  requires P.InvNode(f.fused_parent)
+  requires P.InvNode(f.fused_child)
+  requires B.WFRedirect(IMerge(f))
+  requires B.ValidRedirectNewParent(IMerge(f))
+  ensures B.ValidRedirectNewChildren(IMerge(f))
+  {
+    var r := IMerge(f);
+
+    var left := P.RestrictAndTranslateChild(f.split_parent, f.left_child, f.slot_idx);
+    assert left.pivotTable[0] == f.split_parent.pivotTable[f.slot_idx];
+    assert Last(left.pivotTable) == f.split_parent.pivotTable[f.slot_idx+1];
+
+    var right := P.RestrictAndTranslateChild(f.split_parent, f.right_child, f.slot_idx+1);
+    assert right.pivotTable[0] == f.split_parent.pivotTable[f.slot_idx+1];
+    assert Last(right.pivotTable) == f.split_parent.pivotTable[f.slot_idx+2];
+
+    forall key:Key | key in r.keys 
+    ensures r.old_parent.children[key].ref in r.old_children
+      && var newchild := r.new_children[r.new_parent.children[key].ref];
+      && var oldchild := r.old_children[r.old_parent.children[key].ref];
+      && var edgekey := r.old_parent.children[key].edgeKey; // translated key
+      && newchild.buffer[key] == oldchild.buffer[edgekey]
+      && ((key in newchild.children) <==> (edgekey in oldchild.children))
+      && ((key in newchild.children) ==> newchild.children[key] == oldchild.children[edgekey])
+    {
+      var edgekey := r.old_parent.children[key].edgeKey;
+      assert BoundedKey(f.split_parent.pivotTable, key);
+
+      if (P.G.Keyspace.lt(key, f.pivot)) {
+        RouteIs(f.split_parent.pivotTable, key, f.slot_idx);
+        assert 0 <= f.slot_idx < NumBuckets(f.split_parent.pivotTable); // observe
+        RestrictAndTranslateKeyConsistency(f.split_parent, f.left_child, left, f.slot_idx, key);
+        assert BoundedKey(left.pivotTable, key); // observe
         MergedNodeAndLeftAgree(left, right, f.fused_child, f.pivot, key);
       } else {
-        assert f.split_parent.pivotTable[f.slot_idx+2] == f.fused_parent.pivotTable[f.slot_idx+1];
         RouteIs(f.split_parent.pivotTable, key, f.slot_idx + 1);
-        assert r.old_parent.children[key] == f.right_childref;
-        assert r.old_children[r.old_parent.children[key]] == INode(f.right_child);
-        CutoffNodeAgree(f.right_child, right, f.pivot, ub, key);
+        assert 0 <= f.slot_idx+1 < NumBuckets(f.split_parent.pivotTable); // observe
+        RestrictAndTranslateKeyConsistency(f.split_parent, f.right_child, right, f.slot_idx+1, key);
+        assert BoundedKey(right.pivotTable, key); // observe
         MergedNodeAndRightAgree(left, right, f.fused_child, f.pivot, key);
       }
+    }
+  }
+
+  lemma MergeRefinesRedirectNewGrandChildren(f: P.NodeFusion)
+  requires P.ValidMerge(f)
+  requires P.InvNode(f.split_parent)
+  requires P.InvNode(f.left_child)
+  requires P.InvNode(f.right_child)
+  requires P.InvNode(f.fused_parent)
+  requires P.InvNode(f.fused_child)
+  requires B.WFRedirect(IMerge(f))
+  requires B.ValidRedirectNewParent(IMerge(f))
+  requires B.ValidRedirectNewChildren(IMerge(f))
+  ensures B.ValidRedirectNewGrandchildren(IMerge(f))
+  {
+    var r := IMerge(f);
+
+    var left := P.RestrictAndTranslateChild(f.split_parent, f.left_child, f.slot_idx);
+    assert left.pivotTable[0] == f.split_parent.pivotTable[f.slot_idx];
+    assert Last(left.pivotTable) == f.split_parent.pivotTable[f.slot_idx+1];
+
+    var right := P.RestrictAndTranslateChild(f.split_parent, f.right_child, f.slot_idx+1);
+    assert right.pivotTable[0] == f.split_parent.pivotTable[f.slot_idx+1];
+    assert Last(right.pivotTable) == f.split_parent.pivotTable[f.slot_idx+2];
+
+    assert f.fused_parent.pivotTable[f.slot_idx] == f.split_parent.pivotTable[f.slot_idx];
+    assert f.fused_parent.pivotTable[f.slot_idx+1] == f.split_parent.pivotTable[f.slot_idx+2];
+    assert f.fused_parent.pivotTable[f.slot_idx] == f.fused_child.pivotTable[0];
+    assert f.fused_parent.pivotTable[f.slot_idx+1] == Last(f.fused_child.pivotTable);
+    assert left.pivotTable[0] == f.fused_child.pivotTable[0];
+    assert Last(right.pivotTable) == Last(f.fused_child.pivotTable);
+    
+    assert Keyspace.lte(f.fused_parent.pivotTable[f.slot_idx], f.fused_child.pivotTable[0]);
+    assert Keyspace.lte(Last(f.fused_child.pivotTable), f.fused_parent.pivotTable[f.slot_idx+1]);
+
+    forall edge | edge in IChildren(f.fused_child).Values
+    ensures exists key :: B.ValidRedirectNewGrandchildrenCheckKey(r, key, f.fused_childref, edge.ref)
+    {
+      var _ := MergeRouteNewChild(f, r, f.fused_childref, edge);
+    }
+
+    assert B.ValidRedirectNewGrandchildren(r) by {
+      B.reveal_ValidRedirectNewGrandchildren();
+    }
+  }
+
+  lemma MergeRouteNewChild(f: P.NodeFusion, r: B.Redirect, childref: Reference, edge: B.G.Edge) returns (key: Key)
+  requires P.ValidMerge(f)
+  requires P.InvNode(f.split_parent)
+  requires P.InvNode(f.left_child)
+  requires P.InvNode(f.right_child)
+  requires P.InvNode(f.fused_parent)
+  requires P.InvNode(f.fused_child)
+  requires Keyspace.lte(f.fused_parent.pivotTable[f.slot_idx], f.fused_child.pivotTable[0])
+  requires Keyspace.lte(Last(f.fused_child.pivotTable), f.fused_parent.pivotTable[f.slot_idx+1])
+  requires r == IMerge(f)
+  requires childref in r.new_children
+  requires edge in r.new_children[childref].children.Values
+  ensures B.ValidRedirectNewGrandchildrenCheckKey(r, key, childref, edge.ref)
+  {
+    assert childref == f.fused_childref;
+    var new_child := r.new_children[childref];
+
+    var k :| k in new_child.children && new_child.children[k].ref == edge.ref;
+    var i := Route(f.fused_child.pivotTable, k);
+
+    key := GetKeyInChildBucket(f.fused_parent.pivotTable, f.fused_child.pivotTable, f.slot_idx, i);
   }
 
   lemma RefinesValidMerge(f: P.NodeFusion)
@@ -996,133 +1507,151 @@ module PivotBetreeSpecRefinement {
   {
     var r := IMerge(f);
     PivotBetreeSpecWFNodes.ValidMergeWritesInvNodes(f);
+    assert P.InvNode(P.MergeOps(f)[0].node);
+    assert P.InvNode(P.MergeOps(f)[1].node);
 
-    assert P.WFNode(P.MergeOps(f)[0].node);
-    assert P.WFNode(P.MergeOps(f)[1].node);
+    B.reveal_ValidRedirect();
 
-    assert P.MergeReads(f)[0].node == f.split_parent;
-    assert BucketListWellMarshalled(f.split_parent.buckets);
-
-    forall ref | ref in IMapRestrict(r.old_parent.children, r.keys).Values
-    ensures ref in r.old_childrefs
-    {
-      var key: Key :| IMapsTo(IMapRestrict(r.old_parent.children, r.keys), key, ref);
-      assert key in r.keys;
-      if (P.G.Keyspace.lt(key, f.pivot)) {
-        RouteIs(f.split_parent.pivotTable, key, f.slot_idx);
-        assert ref == f.left_childref;
-      } else {
-        assert f.split_parent.pivotTable[f.slot_idx + 2] == f.fused_parent.pivotTable[f.slot_idx + 1];
-        RouteIs(f.split_parent.pivotTable, key, f.slot_idx+1);
-        assert ref == f.right_childref;
-      }
-    }
-
-    forall ref | ref in r.old_childrefs
-    ensures ref in IMapRestrict(r.old_parent.children, r.keys).Values
-    {
-      assert ref == f.left_childref || ref == f.right_childref;
-      if (ref == f.left_childref) {
-        var key := GetKeyInBucket(f.split_parent.pivotTable, f.slot_idx);
-        RouteIs(f.fused_parent.pivotTable, key, f.slot_idx);
-        assert key in r.keys;
-        assert key in IMapRestrict(r.old_parent.children, r.keys);
-        assert IMapRestrict(r.old_parent.children, r.keys)[key] == ref;
-        assert ref in IMapRestrict(r.old_parent.children, r.keys).Values;
-      } else {
-        var key := GetKeyInBucket(f.split_parent.pivotTable, f.slot_idx + 1);
-        RouteIs(f.fused_parent.pivotTable, key, f.slot_idx);
-        assert key in r.keys;
-        assert key in IMapRestrict(r.old_parent.children, r.keys);
-        assert IMapRestrict(r.old_parent.children, r.keys)[key] == ref;
-        assert ref in IMapRestrict(r.old_parent.children, r.keys).Values;
-      }
-    }
-
-    reveal_MergeBucketsInList();
-    SplitOfMergeBucketsInList(f.split_parent.buckets, f.slot_idx, f.split_parent.pivotTable);
-    SplitMergeBuffersChildrenEq(f.fused_parent, f.split_parent, f.slot_idx);
-
-    // assert redirect.old_children[f.left_childref] == INode(f.left_child);
-    // assert redirect.old_children[f.right_childref] == INode(f.right_child);
-    assert forall k | k in r.keys :: Keyspace.lt(KeyToElement(k), f.fused_parent.pivotTable[f.slot_idx+1]);
-
-    forall key:Key | key in r.keys * r.old_parent.children.Keys
-    ensures r.old_parent.children[key] in r.old_children
-    ensures IMapsAgreeOnKey(r.new_children[r.new_parent.children[key]].buffer, r.old_children[r.old_parent.children[key]].buffer, key)
-    ensures IMapsAgreeOnKey(r.new_children[r.new_parent.children[key]].children, r.old_children[r.old_parent.children[key]].children, key)
-    { MergeChildrenConsistent(f, r, key); }
-
-    forall childref, ref | childref in r.new_children && ref in r.new_children[childref].children.Values
-    ensures exists key ::
-          && IMapsTo(r.new_parent.children, key, childref)
-          && IMapsTo(r.new_children[childref].children, key, ref)
-          && key in r.keys
-          && key in r.old_parent.children
-    { var key := MergeRouteNewChild(f, r, childref, ref); }
+    MergeRefinesWFRedirect(f);
+    MergeRefinesRedirectNewParent(f);
+    MergeRefinesRedirectNewChildren(f);
+    MergeRefinesRedirectNewGrandChildren(f);
   }
 
-  lemma SplitChildrenConsistent(f: P.NodeFusion, r: B.Redirect, key: Key)
+  lemma SplitRefinesWFRedirect(f: P.NodeFusion)
   requires P.ValidSplit(f)
+  requires P.InvNode(f.fused_parent)
+  requires P.InvNode(f.fused_child)
   requires P.InvNode(f.split_parent)
   requires P.InvNode(f.left_child)
   requires P.InvNode(f.right_child)
-  requires P.InvNode(f.fused_parent)
-  requires P.InvNode(f.fused_child)
-  requires r == ISplit(f)
-  requires key in r.keys * r.old_parent.children.Keys
-  ensures r.old_parent.children[key] in r.old_children
-  ensures r.new_parent.children[key] in r.new_children
-  ensures IMapsAgreeOnKey(
-    r.new_children[r.new_parent.children[key]].buffer,
-    r.old_children[r.old_parent.children[key]].buffer, key)
-  ensures IMapsAgreeOnKey(
-    r.new_children[r.new_parent.children[key]].children,
-    r.old_children[r.old_parent.children[key]].children,
-    key)
+  ensures B.WFRedirect(ISplit(f))
   {
-    var lbound := P.getlbound(f.fused_parent, f.slot_idx);
-    var ubound := P.getubound(f.fused_parent, f.slot_idx);
-    var ch := P.CutoffNode(f.fused_child, lbound, ubound);
-    CutoffNodeAgree(f.fused_child, ch, lbound, ubound, key);
+    var r := ISplit(f);
+    var old_parent_children_ref := imap k | k in r.old_parent.children :: r.old_parent.children[k].ref;
 
-    if (P.G.Keyspace.lt(key, f.pivot)) {
-      RouteIs(f.split_parent.pivotTable, key, f.slot_idx);
-      assert r.new_parent.children[key] == f.left_childref;
-      assert r.new_children[r.new_parent.children[key]] == INode(f.left_child);
-      WriteFusedChildInTermsOfLeftAndRight(f.left_child, f.right_child, ch, f.pivot, f.num_children_left);
-      MergedNodeAndLeftAgree(f.left_child, f.right_child, ch, f.pivot, key);
-    } else {
-      if ubound.None? {
-        P.reveal_CutoffNode();
-        P.reveal_CutoffNodeAndKeepRight();
-        assert BoundedKey(f.right_child.pivotTable, key);
-      }
-      assert f.split_parent.pivotTable[f.slot_idx+1] == KeyToElement(f.pivot);
-      assert f.split_parent.pivotTable[f.slot_idx+2] == f.fused_parent.pivotTable[f.slot_idx+1];
-      RouteIs(f.split_parent.pivotTable, key, f.slot_idx+1);
-      assert r.new_parent.children[key] == f.right_childref;
-      assert r.new_children[r.new_parent.children[key]] == INode(f.right_child);
-      WriteFusedChildInTermsOfLeftAndRight(f.left_child, f.right_child, ch, f.pivot, f.num_children_left);
-      MergedNodeAndRightAgree(f.left_child, f.right_child, ch, f.pivot, key);
+    forall ref | ref in r.old_childrefs
+    ensures ref in IMapRestrict(old_parent_children_ref, r.keys).Values
+    {
+      assert ref == f.fused_childref;
+      var key := GetKeyInBucket(f.fused_parent.pivotTable, f.slot_idx);
+      assert IMapRestrict(old_parent_children_ref, r.keys)[key] == ref;
     }
   }
 
-  lemma SplitRouteNewChild(f: P.NodeFusion, r: B.Redirect, childref: Reference, ref: Reference) returns (key: Key)
+  lemma SplitRefinesRedirectNewParent(f: P.NodeFusion)
   requires P.ValidSplit(f)
   requires P.InvNode(f.fused_parent)
   requires P.InvNode(f.fused_child)
+  requires P.InvNode(f.split_parent)
+  requires P.InvNode(f.left_child)
+  requires P.InvNode(f.right_child)
+  requires B.WFRedirect(ISplit(f))
+  ensures B.ValidRedirectNewParent(ISplit(f))
+  {
+    reveal_SplitBucketInList();
+    SplitMergeBuffersChildrenEq(f.fused_parent, f.split_parent, f.slot_idx);
+  }
+
+  lemma SplitRefinesRedirectNewChildren(f: P.NodeFusion)
+  requires P.ValidSplit(f)
+  requires P.InvNode(f.fused_parent)
+  requires P.InvNode(f.fused_child)
+  requires P.InvNode(f.split_parent)
+  requires P.InvNode(f.left_child)
+  requires P.InvNode(f.right_child)
+  requires B.WFRedirect(ISplit(f))
+  requires B.ValidRedirectNewParent(ISplit(f))
+  ensures B.ValidRedirectNewChildren(ISplit(f))
+  {
+    var r := ISplit(f);
+
+    var child := P.RestrictAndTranslateChild(f.fused_parent, f.fused_child, f.slot_idx);
+    assert child.pivotTable[0] == f.fused_parent.pivotTable[f.slot_idx];
+    assert Last(child.pivotTable) == f.fused_parent.pivotTable[f.slot_idx+1];
+    assert Last(f.left_child.pivotTable) == f.right_child.pivotTable[0] == KeyToElement(f.pivot);
+    assert Last(f.right_child.pivotTable) == Last(child.pivotTable);
+
+    WriteFusedChildInTermsOfLeftAndRight(f.left_child, f.right_child, child, f.pivot, f.num_children_left);
+
+    forall key:Key | key in r.keys 
+    ensures r.old_parent.children[key].ref in r.old_children
+      && var newchild := r.new_children[r.new_parent.children[key].ref];
+      && var oldchild := r.old_children[r.old_parent.children[key].ref];
+      && var edgekey := r.old_parent.children[key].edgeKey; // translated key
+      && newchild.buffer[key] == oldchild.buffer[edgekey]
+      && ((key in newchild.children) <==> (edgekey in oldchild.children))
+      && ((key in newchild.children) ==> newchild.children[key] == oldchild.children[edgekey])
+    {
+      var edgekey := r.old_parent.children[key].edgeKey;
+      assert BoundedKey(f.fused_parent.pivotTable, key);
+      assert BoundedKey(f.split_parent.pivotTable, key);
+
+      RestrictAndTranslateKeyConsistency(f.fused_parent, f.fused_child, child, f.slot_idx, key);
+      if (P.G.Keyspace.lt(key, f.pivot)) {
+        RouteIs(f.split_parent.pivotTable, key, f.slot_idx);
+        assert r.new_parent.children[key].ref == f.left_childref;
+        assert r.new_children[r.new_parent.children[key].ref] == INode(f.left_child);
+        MergedNodeAndLeftAgree(f.left_child, f.right_child, child, f.pivot, key);
+      } else {
+        RouteIs(f.split_parent.pivotTable, key, f.slot_idx+1);
+        assert r.new_parent.children[key].ref == f.right_childref;
+        assert r.new_children[r.new_parent.children[key].ref] == INode(f.right_child);
+        WriteFusedChildInTermsOfLeftAndRight(f.left_child, f.right_child, child, f.pivot, f.num_children_left);
+        MergedNodeAndRightAgree(f.left_child, f.right_child, child, f.pivot, key);
+      }
+    }
+  }
+
+  lemma SplitRefinesRedirectNewGrandChildren(f: P.NodeFusion)
+  requires P.ValidSplit(f)
+  requires P.InvNode(f.fused_parent)
+  requires P.InvNode(f.fused_child)
+  requires P.InvNode(f.split_parent)
+  requires P.InvNode(f.left_child)
+  requires P.InvNode(f.right_child)
+  requires B.WFRedirect(ISplit(f))
+  requires B.ValidRedirectNewParent(ISplit(f))
+  requires B.ValidRedirectNewChildren(ISplit(f))
+  ensures B.ValidRedirectNewGrandchildren(ISplit(f))
+  {
+    var r := ISplit(f);
+
+    var child := P.RestrictAndTranslateChild(f.fused_parent, f.fused_child, f.slot_idx);
+    assert child.pivotTable[0] == f.fused_parent.pivotTable[f.slot_idx];
+    assert Last(child.pivotTable) == f.fused_parent.pivotTable[f.slot_idx+1];
+    assert f.fused_parent.pivotTable[f.slot_idx] == f.split_parent.pivotTable[f.slot_idx];
+    assert f.fused_parent.pivotTable[f.slot_idx+1] == f.split_parent.pivotTable[f.slot_idx+2];
+
+    forall childref, edge | childref in r.new_children && edge in r.new_children[childref].children.Values
+    ensures exists key :: B.ValidRedirectNewGrandchildrenCheckKey(r, key, childref, edge.ref)
+    {
+      var _ := SplitRouteNewChild(f, r, childref, edge);
+    }
+
+    assert B.ValidRedirectNewGrandchildren(r) by {
+      B.reveal_ValidRedirectNewGrandchildren();
+    }
+  }
+
+  lemma SplitRouteNewChild(f: P.NodeFusion, r: B.Redirect, childref: Reference, edge: B.G.Edge) returns (key: Key)
+  requires P.ValidSplit(f)
+  requires P.InvNode(f.fused_parent)
+  requires P.InvNode(f.fused_child)
+  requires P.InvNode(f.split_parent)
+  requires P.InvNode(f.left_child)
+  requires P.InvNode(f.right_child)
+  requires Keyspace.lte(f.split_parent.pivotTable[f.slot_idx], f.left_child.pivotTable[0])
+  requires Keyspace.lte(Last(f.left_child.pivotTable), f.split_parent.pivotTable[f.slot_idx+1])
+  requires Keyspace.lte(f.split_parent.pivotTable[f.slot_idx+1], f.right_child.pivotTable[0])
+  requires Keyspace.lte(Last(f.right_child.pivotTable), f.split_parent.pivotTable[f.slot_idx+2])
   requires r == ISplit(f)
   requires childref in r.new_children
-  requires ref in r.new_children[childref].children.Values
-  ensures IMapsTo(r.new_parent.children, key, childref)
-    && IMapsTo(r.new_children[childref].children, key, ref)
-    && key in r.keys
-    && key in r.old_parent.children
+  requires edge in r.new_children[childref].children.Values
+  ensures B.ValidRedirectNewGrandchildrenCheckKey(r, key, childref, edge.ref)
   {
-    PivotBetreeSpecWFNodes.ValidSplitWritesInvNodes(f);
     var new_child := r.new_children[childref];
-    var k :| k in new_child.children && new_child.children[k] == ref;
+    var k :| k in new_child.children && new_child.children[k].ref == edge.ref;
 
     var parent_slot;
     var lr_child;
@@ -1134,16 +1663,8 @@ module PivotBetreeSpecRefinement {
       lr_child := f.right_child;
     }
 
-    ValidLeftChildHasGoodPivots(f);
-    ValidRightChildHasGoodPivots(f);
-
     var child_slot := Route(lr_child.pivotTable, k);
     key := GetKeyInChildBucket(f.split_parent.pivotTable, lr_child.pivotTable, parent_slot, child_slot);
-
-    assert IMapsTo(r.new_parent.children, key, childref);
-    assert IMapsTo(r.new_children[childref].children, key, ref);
-    assert key in r.keys;
-    assert key in r.old_parent.children;
   }
 
   lemma {:timeLimitMultiplier 4} RefinesValidSplit(f: P.NodeFusion)
@@ -1156,45 +1677,201 @@ module PivotBetreeSpecRefinement {
     var r := ISplit(f);
     PivotBetreeSpecWFNodes.ValidSplitWritesInvNodes(f);
 
-    assert P.SplitReads(f)[0].node == f.fused_parent;
-    assert BucketListWellMarshalled(f.fused_parent.buckets);
-    WellMarshalledSplitBucketInList(f.fused_parent.buckets, f.slot_idx,f.pivot);
+    SplitRefinesWFRedirect(f);
+    SplitRefinesRedirectNewParent(f);
+    SplitRefinesRedirectNewChildren(f);
+    SplitRefinesRedirectNewGrandChildren(f);
 
-    // assert (forall ref :: ref in IMapRestrict(r.old_parent.children, r.keys).Values ==> ref in r.old_childrefs);
-    forall ref | ref in r.old_childrefs
-    ensures ref in IMapRestrict(r.old_parent.children, r.keys).Values
+    assert B.ValidRedirect(r) by {
+      B.reveal_ValidRedirect();
+    }
+  }
+
+  lemma RestrictAndTranslateNodeKeyRange(node: PNode, node': PNode, from: Key, to: Key)
+  requires P.WFNode(node)
+  requires ContainsAllKeys(node.pivotTable)
+  requires node.children.Some?
+  requires P.G.Keyspace.lt([], to)
+  requires node' == P.RestrictAndTranslateNode(node, from, to)
+  ensures forall k : Key | IsPrefix(to, k) :: BoundedKey(node'.pivotTable, k)
+  ensures AllKeysInBetweenHasPrefix(node'.pivotTable[0], Last(node'.pivotTable), to)
+  {
+    assert node'.pivotTable[0] == KeyToElement(to);
+    assert Last(node'.pivotTable) == ShortestUncommonPrefix(to, |to|);
+    PrefixOfLcpIsPrefixOfKeys(node'.pivotTable[0], Last(node'.pivotTable), to);
+
+    forall k : Key | IsPrefix(to, k)
+    ensures BoundedKey(node'.pivotTable, k)
     {
-      assert ref == f.fused_childref;
-      var key := GetKeyInBucket(f.fused_parent.pivotTable, f.slot_idx);
-      assert IMapRestrict(r.old_parent.children, r.keys)[key] == ref;
+      reveal_IsPrefix();
+      P.G.Keyspace.EmptyLte(k[|to|..]);
+      PrefixLteProperties(to, to, k);
+      assert Keyspace.lte(node'.pivotTable[0], KeyToElement(k));
+
+      if Last(node'.pivotTable).Element? {
+        Keyspace.reveal_IsStrictlySorted();
+        assert !IsPrefix(to, Last(node'.pivotTable).e);
+        KeyWithPrefixLt(to, Last(node'.pivotTable).e, k);
+      }
+    }
+  }
+
+  lemma RestrictAndTranslateNodePreservesChildren(node: PNode, node': PNode, from: Key, to: Key, key: Key, key': Key)
+  requires P.InvNode(node)
+  requires ContainsAllKeys(node.pivotTable)
+  requires node.children.Some?
+  requires P.G.Keyspace.lt([], to)
+  requires node' == P.RestrictAndTranslateNode(node, from, to)
+  requires IsPrefix(to, key')
+  requires BoundedKey(node.pivotTable, key)
+  requires BoundedKey(node'.pivotTable, key')
+  requires key == from + key'[|to|..]
+  ensures IChildren(node)[key] == IChildren(node')[key']
+  {
+    var fromend := ShortestUncommonPrefix(from, |from|);
+    var fromendkey := if fromend.Element? then (var k : Key := fromend.e; Some(k)) else None;
+
+    ContainsAllKeysImpliesBoundedKey(node.pivotTable, from);
+    var fromnode := P.CutoffNode(node, from, fromendkey);
+
+    P.G.Keyspace.EmptyLte(key[|from|..]);
+    PrefixLteProperties(from, from, key);
+    if fromendkey.Some? {
+      KeyWithPrefixLt(from, fromendkey.value, key);
     }
 
-    reveal_SplitBucketInList();
-    SplitMergeBuffersChildrenEq(f.fused_parent, f.split_parent, f.slot_idx);
+    CutoffNodeAgree(node, fromnode, from, fromendkey, key);
+    assert IChildren(node)[key] == IChildren(fromnode)[key];
 
-    forall childref, ref | childref in r.new_children && ref in r.new_children[childref].children.Values
-    ensures exists key ::
-          && IMapsTo(r.new_parent.children, key, childref)
-          && IMapsTo(r.new_children[childref].children, key, ref)
-          && key in r.keys
-          && key in r.old_parent.children
-    { var key := SplitRouteNewChild(f, r, childref, ref); }
+    var toend := ShortestUncommonPrefix(to, |to|);
+    assert node'.pivotTable[0] == KeyToElement(to);
+    assert Last(node'.pivotTable) == toend;
+    assert PivotLcp(node'.pivotTable[0], Last(node'.pivotTable)) == to;
 
-    forall key:Key | key in r.keys * r.old_parent.children.Keys
-    ensures r.old_parent.children[key] in r.old_children
-    ensures r.new_parent.children[key] in r.new_children
-    ensures IMapsAgreeOnKey(
-          r.new_children[r.new_parent.children[key]].buffer,
-          r.old_children[r.old_parent.children[key]].buffer,
-          key)
-    ensures IMapsAgreeOnKey(
-          r.new_children[r.new_parent.children[key]].children,
-          r.old_children[r.old_parent.children[key]].children,
-          key)
-    { SplitChildrenConsistent(f, r, key); }
+    TranslatePivotsSameRoute(fromnode.pivotTable, node'.pivotTable, from, to, key, key');
+    TranslatePivotsEdgesPreserveTranslateKey(fromnode.pivotTable, fromnode.edgeTable,
+      node'.pivotTable, node'.edgeTable, from, to, Last(node'.pivotTable), key, key');
+  }
 
-    assert (forall ref :: ref in IMapRestrict(r.new_parent.children, r.keys).Values ==> ref in r.new_childrefs);
-    assert r.new_children.Keys == (iset ref | ref in r.new_childrefs);
+  predicate IsNodeSlice(node: PNode, subnode: PNode, a: int, b: int)
+  {
+    && P.WFNode(node)
+    && P.WFNode(subnode)
+    && 0 <= a < b < |node.pivotTable|
+    && |subnode.buckets| <= |node.buckets|
+    && node.pivotTable[a..b+1] == subnode.pivotTable
+    && node.edgeTable[a..b] == subnode.edgeTable
+    && node.buckets[a..b] == subnode.buckets
+    && (node.children.Some? <==> subnode.children.Some?)
+    && (node.children.Some? ==> node.children.value[a..b] == subnode.children.value)
+  }
+
+  lemma NodeSliceProperty(node: PNode, subnode: PNode, key: Key, a: int, b: int)
+  requires IsNodeSlice(node, subnode, a, b)
+  requires BoundedKey(node.pivotTable, key)
+  requires BoundedKey(subnode.pivotTable, key)
+  ensures IBuffer(node)[key] == IBuffer(subnode)[key]
+  ensures node.children.Some? ==> IChildren(node)[key] == IChildren(subnode)[key]
+  {
+    var r := Route(node.pivotTable, key);
+    var r' := Route(subnode.pivotTable, key);
+    assert r' == r - a;
+    if node.children.Some? {
+      assert node.children.value[r] == subnode.children.value[r'];
+    }
+  }
+
+  lemma RefinesValidClone(clone: P.NodeClone)
+  requires P.ValidClone(clone)
+  requires forall i | 0 <= i < |P.CloneReads(clone)| :: P.InvNode(P.CloneReads(clone)[i].node)
+  requires ReadOpsBucketsWellMarshalled(P.CloneReads(clone))
+  ensures B.ValidClone(IClone(clone))
+  {
+    var c := IClone(clone);
+    PivotBetreeSpecWFNodes.ValidCloneWritesInvNodes(clone);
+    assert P.InvNode(P.CloneReads(clone)[0].node);
+
+    ContainsAllKeysImpliesBoundedKey(clone.oldroot.pivotTable, clone.from);
+    var rstart := Route(clone.oldroot.pivotTable, clone.from);
+    var fromend := ShortestUncommonPrefix(clone.from, |clone.from|);
+    var rend := if fromend.Max_Element? then |clone.oldroot.buckets| 
+        else Route(clone.oldroot.pivotTable, fromend.e) + 1;
+    assert BucketListNoKeyWithPrefix(clone.oldroot.buckets[rstart..rend], clone.from);
+
+    forall k | k in c.new_to_old
+    ensures IMapsTo(c.oldroot.buffer, c.new_to_old[k], Update(NopDelta()))
+    ensures c.new_to_old[k] in c.oldroot.children
+    {
+      ContainsAllKeysImpliesBoundedKey(clone.oldroot.pivotTable, c.new_to_old[k]);
+      var key : Key := c.new_to_old[k];
+      var r := Route(clone.oldroot.pivotTable, key);
+
+      Keyspace.Base_Order.EmptyLte(key[|clone.from|..]);
+      PrefixLteProperties(clone.from, clone.from, key);
+      assert Keyspace.lte(KeyToElement(clone.from), KeyToElement(key));
+
+      if fromend.Element? {
+        KeyWithPrefixLt(clone.from, fromend.e, key);
+        assert r <= rend;
+      }
+
+      assert clone.oldroot.buckets[rstart..rend][r-rstart] == clone.oldroot.buckets[r];
+      assert BucketNoKeyWithPrefix(clone.oldroot.buckets[r], clone.from);
+      MapSeqs.key_sets_eq(clone.oldroot.buckets[r].keys, clone.oldroot.buckets[r].msgs);
+    }
+
+    // new root condition - keys affected by clone
+    ContainsAllKeysImpliesBoundedKey(clone.oldroot.pivotTable, clone.to);
+    var lnode := P.CutoffNodeAndKeepLeft(clone.oldroot, clone.to);
+    assert Last(lnode.pivotTable) == KeyToElement(clone.to);
+    assert |lnode.pivotTable| < |clone.newroot.pivotTable|;
+
+    var tonode := P.RestrictAndTranslateNode(clone.oldroot, clone.from, clone.to);
+    RestrictAndTranslateNodeKeyRange(clone.oldroot, tonode, clone.from, clone.to);
+
+    var tostart := |lnode.buckets|;
+    var toend := |lnode.buckets|+|tonode.buckets|;
+    assert IsNodeSlice(clone.newroot, tonode, tostart, toend);
+
+    forall k | k in c.new_to_old
+    ensures IMapsTo(c.newroot.buffer, k, Update(NopDelta()))
+    ensures IMapsTo(c.newroot.children, k, c.oldroot.children[c.new_to_old[k]])
+    {
+      RestrictAndTranslateNodePreservesChildren(clone.oldroot, tonode, clone.from, clone.to, c.new_to_old[k], k);
+      ContainsAllKeysImpliesBoundedKey(clone.newroot.pivotTable, k);
+      NodeSliceProperty(clone.newroot, tonode, k, tostart, toend);
+    }
+
+    // new root condition - keys not affected by clone
+    assert clone.newroot.pivotTable[..tostart] == lnode.pivotTable[..tostart];
+    assert clone.newroot.pivotTable[tostart] == KeyToElement(clone.to);
+    assert IsNodeSlice(clone.newroot, lnode, 0, tostart);
+
+    var rnode : PNode;
+    var toendkey : Key;
+    if Last(tonode.pivotTable).Element? {
+      toendkey := GetKey(tonode.pivotTable, |tonode.pivotTable|-1);
+      rnode := P.CutoffNodeAndKeepRight(clone.oldroot, toendkey);
+      assert IsNodeSlice(clone.newroot, rnode, toend, |clone.newroot.buckets|);
+    }
+
+    forall k : Key | k !in c.new_to_old
+    ensures IMapsAgreeOnKey(c.newroot.buffer, c.oldroot.buffer, k)
+    ensures IMapsAgreeOnKey(c.newroot.children, c.oldroot.children, k)
+    {
+      ContainsAllKeysImpliesBoundedKey(clone.oldroot.pivotTable, k);
+      ContainsAllKeysImpliesBoundedKey(clone.newroot.pivotTable, k);
+      var r := Route(clone.newroot.pivotTable, k);
+      assert r < tostart || r >= toend;
+
+      if r < tostart {
+        CutoffNodeAndKeepLeftAgree(clone.oldroot, lnode, clone.to, k);
+        NodeSliceProperty(clone.newroot, lnode, k, 0, tostart);
+      } else {
+        CutoffNodeAndKeepRightAgree(clone.oldroot, rnode, toendkey, k);
+        NodeSliceProperty(clone.newroot, rnode, k, toend, |clone.newroot.buckets|);
+      }
+    }
   }
 
   lemma RefinesValidBetreeStep(betreeStep: P.BetreeStep)
@@ -1221,6 +1898,16 @@ module PivotBetreeSpecRefinement {
         assert P.InvNode(P.BetreeStepReads(betreeStep)[2].node);
         RefinesValidMerge(fusion);
       }
+      case BetreeClone(clone) => RefinesValidClone(clone);
+    }
+  }
+
+  lemma IReadOpsEquiv(lookup: P.Lookup)
+  requires forall i | 0 <= i < |lookup| :: P.WFNode(lookup[i].readOp.node)
+  ensures IReadOps(P.LayersToReadOps(lookup)) == B.LayersToReadOps(ILayers(lookup));
+  {
+    if |lookup| > 0 {
+      IReadOpsEquiv(DropLast(lookup));
     }
   }
 
@@ -1235,6 +1922,11 @@ module PivotBetreeSpecRefinement {
     B.reveal_RedirectReads();
     B.reveal_RedirectOps();
     RefinesValidBetreeStep(betreeStep);
+
+    if betreeStep.BetreeQuery? || betreeStep.BetreeSuccQuery? {
+      var lookup := if betreeStep.BetreeQuery? then betreeStep.q.lookup else betreeStep.sq.lookup;
+      IReadOpsEquiv(lookup);
+    }
   }
 
   // interpret the pivot-y Ops (from our little cache DSL) to their Betree (non-pivot) versions.
@@ -1294,29 +1986,7 @@ module PivotBetreeSpecRefinement {
 
     assert INode(newroot).children == newroot'.children;
     assert INode(newroot).buffer == newroot'.buffer;
-
     assert INode(newroot) == newroot';
-  }
-
-  lemma AddMessagesToNodeResult(node: PNode, bucket: BucketMap, node': PNode, key: Key)
-  requires P.InvNode(node)
-  requires P.WFNode(node')
-  requires WFBucketListProper(node'.buckets, node'.pivotTable);
-  requires BucketListWellMarshalled(node.buckets)
-  requires BoundedKey(node.pivotTable, key)
-  requires BoundedKey(node'.pivotTable, key)
-  requires node'.pivotTable == node.pivotTable
-  requires node'.children == node.children
-  requires MapsOfBucketList(node'.buckets)
-      == BucketListFlush(bucket, MapsOfBucketList(node.buckets), node.pivotTable)
-  ensures WFBucketListProper(node'.buckets, node'.pivotTable);
-  ensures key !in bucket ==> P.NodeLookup(node', key) == P.NodeLookup(node, key)
-  ensures key in bucket ==> P.NodeLookup(node', key) == Merge(bucket[key], P.NodeLookup(node, key))
-  {
-    //GetBucketListFlushEqMerge(bucket, node.buckets, node.pivotTable, key);
-    var i := Route(node.pivotTable, key);
-    assert node'.buckets[i].as_map() == 
-        BucketListItemFlush(bucket, node.buckets[i].as_map(), node.pivotTable, i);
   }
 
   lemma {:fuel IOps,2} FlushRefinesOps(flush: P.NodeFlush)
@@ -1341,19 +2011,12 @@ module PivotBetreeSpecRefinement {
     assert P.InvNode(P.GrowReads(growth)[0].node);
     PivotBetreeSpecWFNodes.ValidGrowWritesInvNodes(growth);
 
-    var newroot := P.G.Node(InitPivotTable(), Some([growth.newchildref]), [BucketsLib.EmptyBucket()]);
+    var newroot := P.G.Node(InitPivotTable(), [None], Some([growth.newchildref]), [EmptyBucket()]);
     P.PivotsHasAllKeys(newroot.pivotTable);
 
     // observe: (I don't know really know why this is necessary)
     assert B.GrowOps(IGrow(growth))[1] 
         == B.G.WriteOp(B.G.Root(), INode(newroot));
-    /*
-    assert IOps(P.GrowOps(growth))
-        == IOps([P.G.AllocOp(growth.newchildref, growth.oldroot), P.G.WriteOp(P.G.Root(), newroot)])
-        == [B.G.AllocOp(growth.newchildref, INode(growth.oldroot)), B.G.WriteOp(B.G.Root(), INode(newroot))]
-        == [B.G.AllocOp(IGrow(growth).newchildref, IGrow(growth).oldroot), B.G.WriteOp(B.G.Root(), newroot')]
-        == B.GrowOps(IGrow(growth));
-    */
   }
 
   lemma {:fuel IOps,3} SplitRefinesOps(f: P.NodeFusion)
@@ -1411,6 +2074,17 @@ module PivotBetreeSpecRefinement {
     PivotBetreeSpecWFNodes.ValidMergeWritesInvNodes(f);
   }
 
+  lemma {:fuel IOps,3} CloneRefinesOps(c: P.NodeClone)
+  requires P.ValidClone(c)
+  requires P.InvNode(c.oldroot)
+  requires B.ValidClone(IClone(c))
+  ensures forall i | 0 <= i < |P.CloneOps(c)| ::
+      P.InvNode(P.CloneOps(c)[i].node)
+  ensures IOps(P.CloneOps(c)) == B.CloneOps(IClone(c))
+  {
+    PivotBetreeSpecWFNodes.ValidCloneWritesInvNodes(c);
+  }
+
   // The meaty lemma: If we mutate the nodes of a pivot-y cache according to a
   // (generic-DSL) BetreeStep, under the INode interpretation, the same
   // mutation happens to the imap-y cache.
@@ -1457,23 +2131,27 @@ module PivotBetreeSpecRefinement {
         assert P.InvNode(P.BetreeStepReads(betreeStep)[2].node);
         MergeRefinesOps(fusion);
       }
+      case BetreeClone(clone) => {
+        assert P.InvNode(P.BetreeStepReads(betreeStep)[0].node);
+        CloneRefinesOps(clone);
+      }
     }
   }
 
-  /*lemma IBufferLeafEqJoin(node: PNode)
-  requires P.InvNode(node)
-  requires BucketListWellMarshalled(node.buckets)
-  ensures IBufferLeaf(node) == imap key :: if BoundedKey(node.pivotTable, key) then Merge(BucketGet(JoinBucketList(node.buckets), key), DefineDefault()) else DefineDefault() 
-  {
-    forall key:Key | BoundedKey(node.pivotTable, key)
-    ensures IBufferLeaf(node)[key] == Merge(BucketGet(JoinBucketList(node.buckets), key), DefineDefault())
-    {
-      forall i | 0 <= i < |node.buckets| ensures WFBucketAt(node.buckets[i], node.pivotTable, i)
-      {
-      }
-      GetJoinBucketListEq(node.buckets, node.pivotTable, key);
-    }
-  }*/
+  // /*lemma IBufferLeafEqJoin(node: PNode)
+  // requires P.InvNode(node)
+  // requires BucketListWellMarshalled(node.buckets)
+  // ensures IBufferLeaf(node) == imap key :: if BoundedKey(node.pivotTable, key) then Merge(BucketGet(JoinBucketList(node.buckets), key), DefineDefault()) else DefineDefault() 
+  // {
+  //   forall key:Key | BoundedKey(node.pivotTable, key)
+  //   ensures IBufferLeaf(node)[key] == Merge(BucketGet(JoinBucketList(node.buckets), key), DefineDefault())
+  //   {
+  //     forall i | 0 <= i < |node.buckets| ensures WFBucketAt(node.buckets[i], node.pivotTable, i)
+  //     {
+  //     }
+  //     GetJoinBucketListEq(node.buckets, node.pivotTable, key);
+  //   }
+  // }*/
 
   lemma RepivotPreservesNode(r: P.Repivot)
   requires P.ValidRepivot(r)
@@ -1517,10 +2195,10 @@ module PivotBetreeSpecRefinement {
     JoinBucketsSplitBucketOnPivotsCancel(joined, r.pivots);
     assert JoinBucketList(buckets1) == JoinBucketList(buckets2);
     
-    IBufferLeafEqJoin(r.leaf);
-    IBufferLeafEqJoin(P.ApplyRepivot(r));
+  //   IBufferLeafEqJoin(r.leaf);
+  //   IBufferLeafEqJoin(P.ApplyRepivot(r));
 
-    BoundedBucketListJoin(buckets1, r.leaf.pivotTable);
-    assert BoundedBucket(joined, r.leaf.pivotTable);*/
+  //   BoundedBucketListJoin(buckets1, r.leaf.pivotTable);
+  //   assert BoundedBucket(joined, r.leaf.pivotTable);*/
   }
 }
