lib/Buckets/TranslationLib.i.dfy
@@ -1,0 +1,1097 @@
+include "BoundedPivotsLib.i.dfy"
+include "BucketsLib.i.dfy"
+include "MapSeqs.i.dfy"
+
+include "../Base/KeyType.s.dfy"
+include "../Lang/System/SeqComparison.s.dfy"
+
+//
+// Provides definitions and libraries for edge table and 
+// other translation related functions and lemma
+//
+
+module TranslationLib {
+  import opened NativeTypes
+  import opened BoundedPivotsLib
+  import opened BucketsLib
+  import opened MapSeqs
+  import opened Sequences
+  import opened Options
+  import opened KeyType
+
+  import SeqComparison
+
+  type EdgeTable = seq<Option<Key>>
+
+  predicate NonEmptyLcp(pt: PivotTable, i: int)
+  requires WFPivots(pt)
+  requires 0 <= i < NumBuckets(pt)
+  {
+    Keyspace.reveal_IsStrictlySorted();
+    PivotLcp(pt[i], pt[i+1]) != []
+  }
+
+  predicate WFEdges(et: EdgeTable, pt: PivotTable)
+  requires WFPivots(pt)
+  {
+    && |et| == NumBuckets(pt)
+    && (forall i | 0 <= i < |et| && et[i].Some? :: NonEmptyLcp(pt, i))
+  }
+
+  predicate TranslationPreserved(pt: PivotTable, et: EdgeTable, pt': PivotTable, et': EdgeTable)
+  requires WFPivots(pt)
+  requires WFPivots(pt')
+  requires WFEdges(et, pt)
+  requires WFEdges(et', pt')
+  {
+    && (forall key | BoundedKey(pt', key) :: 
+        && BoundedKey(pt, key)
+        && TranslateKey(pt', et', key) == TranslateKey(pt, et, key))
+  }
+
+  function SplitLeftEdges(et: EdgeTable, pt: PivotTable, pivot: Key) : (et': EdgeTable)
+  requires WFPivots(pt)
+  requires WFEdges(et, pt)
+  requires ValidLeftCutOffKey(pt, pivot)
+  ensures WFEdges(et', SplitLeft(pt, pivot))
+  ensures TranslationPreserved(pt, et, SplitLeft(pt, pivot), et')
+  {
+    var cLeft := CutoffForLeft(pt, pivot);
+    if (pt[cLeft + 1].Element? && pt[ cLeft+1 ].e == pivot) || et[cLeft].None? then (
+      et[..cLeft + 1]
+    ) else (
+      var pt' := SplitLeft(pt, pivot);
+
+      var oldlcp : Key := PivotLcp(pt[cLeft], pt[cLeft+1]);
+      var newlcp : Key := PivotLcp(pt'[cLeft], pt'[cLeft+1]);
+      PivotLcpSubRangeLeft(pt[cLeft], pt[cLeft+1], pt'[cLeft+1]);
+  
+      assume |et[cLeft].value + newlcp[|oldlcp|..]| <= 1024;
+      var translation : Key := et[cLeft].value + newlcp[|oldlcp|..];
+      var et' := et[..cLeft] +  [Some(translation)];
+
+      assert TranslationPreserved(pt, et, pt', et') by {
+        forall key | BoundedKey(pt', key)
+        ensures BoundedKey(pt, key)
+        ensures TranslateKey(pt', et', key) == TranslateKey(pt, et, key)
+        {
+          var i := Route(pt, key);
+          if i == cLeft {
+            assert pt[cLeft] == pt'[cLeft];
+            assert TranslateKey(pt', et', key) == TranslateKey(pt, et, key);
+          }
+        }
+      }
+
+      et'
+    )
+  }
+
+  function SplitRightEdges(et: EdgeTable, pt: PivotTable, pivot: Key) : (et': EdgeTable)
+  requires WFPivots(pt)
+  requires WFEdges(et, pt)
+  requires BoundedKey(pt, pivot)
+  ensures WFEdges(et', SplitRight(pt, pivot))
+  ensures TranslationPreserved(pt, et, SplitRight(pt, pivot), et')
+  {
+    var cRight := CutoffForRight(pt, pivot);
+    if pt[cRight].e == pivot || et[cRight].None? then (
+      et[cRight..]
+    ) else (
+      var pt' := SplitRight(pt, pivot);
+
+      var oldlcp : Key := PivotLcp(pt[cRight], pt[cRight+1]);
+      var newlcp : Key := PivotLcp(pt'[0], pt'[1]);
+      PivotLcpSubRangeRight(pt[cRight], pt'[0], pt'[1]);
+
+      assume |et[cRight].value + newlcp[|oldlcp|..]| <= 1024;
+      var translation : Key := et[cRight].value + newlcp[|oldlcp|..];
+      var et' := [Some(translation)] + et[cRight+1..];
+
+      assert TranslationPreserved(pt, et, pt', et') by {
+        forall key | BoundedKey(pt', key)
+        ensures BoundedKey(pt, key)
+        ensures TranslateKey(pt', et', key) == TranslateKey(pt, et, key)
+        {
+          var i := Route(pt, key);
+          if i == cRight {
+            assert pt[cRight+1] == pt'[1];
+            assert TranslateKey(pt', et', key) == TranslateKey(pt, et, key);
+          }
+        }
+      }
+
+      et'
+    )
+  }
+
+  lemma WFConcatEdges(leftpt: PivotTable, leftet: EdgeTable, rightpt: PivotTable, rightet: EdgeTable, pt: PivotTable)
+  requires WFPivots(leftpt)
+  requires WFPivots(rightpt)
+  requires WFPivots(pt)
+  requires WFEdges(leftet, leftpt)
+  requires WFEdges(rightet, rightpt)
+  requires Last(leftpt) == rightpt[0]
+  requires pt == concat3(leftpt[..|leftpt|-1], Last(leftpt), rightpt[1..])
+  ensures WFEdges(concat(leftet, rightet), pt)
+  ensures TranslationPreserved(pt, concat(leftet, rightet), leftpt, leftet)
+  ensures TranslationPreserved(pt, concat(leftet, rightet), rightpt, rightet)
+  {
+    var et := concat(leftet, rightet);
+    assert |et| == NumBuckets(pt);
+
+    forall i | 0 <= i < |et|
+    ensures et[i].Some? ==> PivotLcp(pt[i], pt[i+1]) != []
+    {
+      if i < |leftet| {
+        assert pt[i] == leftpt[i];
+        assert pt[i+1] == leftpt[i+1];
+        assert et[i] == leftet[i];
+      } else {
+        assert pt[i] == rightpt[i-|leftet|];
+        assert pt[i+1] == rightpt[i-|leftet|+1];
+        assert et[i] == rightet[i-|leftet|];
+      }
+    }
+    Keyspace.reveal_IsStrictlySorted();
+  }
+
+  // lcp functions and lemma
+
+  function lcpright(left: Key): (prefix: Key)
+  ensures IsPrefix(prefix, left)
+  ensures SeqComparison.lte(prefix, left)
+  {
+    reveal_IsPrefix();
+    SeqComparison.reveal_lte();
+
+    if |left| > 0 && left[0] as int == Uint8UpperBound() as int - 1 then
+      [left[0]] + lcpright(left[1..])
+    else
+      []
+  }
+
+  function lcp(left: Key, right: Key): (prefix: Key)
+  ensures IsPrefix(prefix, left)
+  ensures SeqComparison.lte(prefix, left)
+  {
+    reveal_IsPrefix();
+    SeqComparison.reveal_lte();
+
+    if |left| > 0 && |right| > 0 && left[0] == right[0] then (
+      [left[0]] + lcp(left[1..], right[1..])
+    ) else if |left| > 0 && |right| == 1 && (left[0] as int + 1) == right[0] as int then (
+      [left[0]] + lcpright(left[1..])
+    ) else (
+      []
+    )
+  }
+
+  function PivotLcp(left: Element, right: Element) : (prefix: Key)
+  requires ElementIsKey(left)
+  requires right.Element? ==> ElementIsKey(right)
+  {
+    if right.Max_Element? then (
+      lcpright(left.e)
+    ) else (
+      lcp(left.e, right.e)
+    )
+  }
+
+  lemma lcprightCorrect(left: Key, prefix: Key, key: Key)
+  requires lcpright(left) == prefix
+  requires SeqComparison.lte(left, key)
+  ensures IsPrefix(prefix, key)
+  {
+    reveal_IsPrefix();
+    SeqComparison.reveal_lte();
+
+    if |left| > 0 && left[0] as int == Uint8UpperBound() as int - 1 {
+      lcprightCorrect(left[1..], prefix[1..], key[1..]);
+    }
+  }
+
+  lemma lcprightSubRangeRight(left: Key, left': Key, prefix: Key, prefix': Key)
+  requires lcpright(left) == prefix
+  requires lcpright(left') == prefix'
+  requires SeqComparison.lte(left, left')
+  ensures IsPrefix(prefix, prefix')
+  {
+    reveal_IsPrefix();
+    SeqComparison.reveal_lte();
+
+    if |left| > 0 && left[0] as int == Uint8UpperBound() as int - 1 {
+      lcprightSubRangeRight(left[1..], left'[1..], prefix[1..], prefix'[1..]);
+    }
+  }
+
+  lemma lcprightSubRangeLeft(left: Key, right: Key, prefix: Key, prefix': Key)
+  requires lcpright(left) == prefix
+  requires lcp(left, right) == prefix'
+  requires SeqComparison.lt(left, right)
+  ensures IsPrefix(prefix, prefix')
+  {
+    reveal_IsPrefix();
+    SeqComparison.reveal_lte();
+
+    if |left| > 0 && left[0] as int == Uint8UpperBound() as int - 1 {
+      lcprightSubRangeLeft(left[1..], right[1..], prefix[1..], prefix'[1..]);
+    }
+  }
+
+  lemma lcpCorrect(left: Key, right: Key, prefix: Key, key: Key)
+  requires lcp(left, right) == prefix
+  requires SeqComparison.lte(left, key)
+  requires SeqComparison.lt(key, right)
+  ensures IsPrefix(prefix, key)
+  {
+    reveal_IsPrefix();
+    SeqComparison.reveal_lte();
+
+    if |left| > 0 && |right| > 0 && left[0] == right[0] {
+      lcpCorrect(left[1..], right[1..], prefix[1..], key[1..]);
+    } else if |left| > 0 && |right| == 1 && (left[0] as int + 1) == right[0] as int {
+      if key[0] == right[0] {
+        assert SeqComparison.lt(key[1..], right[1..]);
+        assert false;
+      }
+      lcprightCorrect(left[1..], lcpright(left[1..]), key[1..]);
+    }
+  }
+
+  lemma lcpSubRangeRight(left: Key, left': Key, right: Key, prefix: Key, prefix': Key)
+  requires lcp(left, right) == prefix
+  requires lcp(left', right) == prefix'
+  requires SeqComparison.lte(left, left')
+  requires SeqComparison.lt(left', right)
+  ensures IsPrefix(prefix, prefix')
+  {
+    reveal_IsPrefix();
+    SeqComparison.reveal_lte();
+
+    if |left| > 0 && |right| > 0 && left[0] == right[0] {
+      lcpSubRangeRight(left[1..], left'[1..], right[1..], prefix[1..], prefix'[1..]);
+    } else if |left| > 0 && |right| == 1 && (left[0] as int + 1) == right[0] as int {
+      if left'[0] == right[0] {
+        assert SeqComparison.lt(left'[1..], right[1..]);
+        assert false;
+      }
+      lcprightSubRangeRight(left[1..], left'[1..], prefix[1..], prefix'[1..]);
+    }
+  }
+
+  lemma lcpSubRangeLeft(left: Key, right: Key, right': Key, prefix: Key, prefix': Key)
+  requires lcp(left, right) == prefix
+  requires lcp(left, right') == prefix'
+  requires SeqComparison.lt(right', right)
+  requires SeqComparison.lt(left, right')
+  ensures IsPrefix(prefix, prefix')
+  {
+    reveal_IsPrefix();
+    SeqComparison.reveal_lte();
+
+    if |left| > 0 && |right| > 0 && left[0] == right[0] {
+      lcpSubRangeLeft(left[1..], right[1..], right'[1..], prefix[1..], prefix'[1..]);
+    } else if |left| > 0 && |right| == 1 && (left[0] as int + 1) == right[0] as int {
+      if right'[0] == right[0] {
+        assert SeqComparison.lt(right'[1..], right[1..]);
+        assert false;
+      }
+      lcprightSubRangeLeft(left[1..], right'[1..], prefix[1..], prefix'[1..]);
+    }
+  }
+
+  lemma PivotLcpSubRangeRight(left: Element, left': Element, right: Element)
+  requires ElementIsKey(left)
+  requires ElementIsKey(left')
+  requires Keyspace.lte(left, left')
+  requires Keyspace.lt(left', right)
+  requires right.Element? ==> ElementIsKey(right)
+  ensures IsPrefix(PivotLcp(left, right), PivotLcp(left', right))
+  {
+    var oldprefix := PivotLcp(left, right);
+    var newprefix := PivotLcp(left', right);
+
+    if right.Max_Element? {
+      lcprightSubRangeRight(left.e, left'.e, oldprefix, newprefix);
+    } else {
+      lcpSubRangeRight(left.e, left'.e, right.e, oldprefix, newprefix);
+    }
+  }
+
+  lemma PivotLcpSubRangeLeft(left: Element, right: Element, right': Element)
+  requires ElementIsKey(left)
+  requires ElementIsKey(right')
+  requires Keyspace.lt(left, right')
+  requires Keyspace.lt(right', right)
+  requires right.Element? ==> ElementIsKey(right)
+  ensures IsPrefix(PivotLcp(left, right), PivotLcp(left, right'))
+  {
+    var oldprefix := PivotLcp(left, right);
+    var newprefix := PivotLcp(left, right');
+
+    if right.Max_Element? {
+      lcprightSubRangeLeft(left.e, right'.e, oldprefix, newprefix);
+    } else {
+      lcpSubRangeLeft(left.e, right.e, right'.e, oldprefix, newprefix);
+    }
+  }
+
+  lemma PrefixOfLcpIsPrefixOfKey(left: Element, right: Element, prefix: Key, key: Key)
+  requires ElementIsKey(left)
+  requires right.Element? ==> ElementIsKey(right)
+  requires Keyspace.lt(left, right)
+  requires InBetween(left, right, key)
+  requires IsPrefix(prefix, PivotLcp(left, right))
+  ensures IsPrefix(prefix, key)
+  {
+    reveal_IsPrefix();
+    SeqComparison.reveal_lte();
+
+    var lcp := PivotLcp(left, right);
+    if right.Max_Element? {
+      Keyspace.Base_Order.transitivity(lcp, left.e, key);
+      lcprightCorrect(left.e, lcp, key);
+    } else {
+      lcpCorrect(left.e, right.e, lcp, key);
+    }
+  }
+
+  lemma PrefixOfLcpIsPrefixOfKeys(left: Element, right: Element, prefix: Key)
+  requires ElementIsKey(left)
+  requires right.Element? ==> ElementIsKey(right)
+  requires Keyspace.lt(left, right)
+  requires IsPrefix(prefix, PivotLcp(left, right))
+  ensures AllKeysInBetweenHasPrefix(left, right, prefix)
+  {
+    forall key : Key | InBetween(left, right, key)
+    ensures IsPrefix(prefix, key)
+    {
+      PrefixOfLcpIsPrefixOfKey(left, right, prefix, key);
+    }
+  }
+
+  predicate AllKeysInBetweenHasPrefix(left: Element, right: Element, prefix: Key)
+  requires ElementIsKey(left)
+  requires right.Element? ==> ElementIsKey(right)
+  requires Keyspace.lt(left, right)
+  {
+    && (forall key : Key | InBetween(left, right, key) :: IsPrefix(prefix, key))
+  }
+
+  // used by succ query
+  datatype PrefixSet = PrefixSet(prefix: Key, newPrefix: Key)
+  type TranslationTable = seq<Option<PrefixSet>>
+
+  function Translate(pt: PivotTable, et: EdgeTable, key: Key): (pset: Option<PrefixSet>)
+  requires WFPivots(pt)
+  requires BoundedKey(pt, key)
+  requires WFEdges(et, pt)
+  ensures pset.Some? ==> IsPrefix(pset.value.prefix, key)
+  {
+    var r := Route(pt, key);
+    if et[r].None? then
+      None
+    else
+      var prefix := PivotLcp(pt[r], pt[r+1]);
+      PrefixOfLcpIsPrefixOfKey(pt[r], pt[r+1], prefix, key);
+      Some(PrefixSet(prefix, et[r].value))
+  }
+
+  function TranslateKey(pt: PivotTable, et: EdgeTable, key: Key): Key
+  requires WFPivots(pt)
+  requires BoundedKey(pt, key)
+  requires WFEdges(et, pt)
+  {
+    var pset := Translate(pt, et, key);
+    ApplyPrefixSet(pset, key)
+  }
+
+  function RevPrefixSet(pset: Option<PrefixSet>) : Option<PrefixSet>
+  {
+    if pset.None? then None else Some(PrefixSet(pset.value.newPrefix, pset.value.prefix))
+  }
+
+  function method ApplyPrefixSet(pset: Option<PrefixSet>, key: Key) : (key': Key)
+  requires pset.Some? ==> IsPrefix(pset.value.prefix, key)
+  ensures pset.Some? ==> IsPrefix(pset.value.newPrefix, key')
+  {
+    if pset.None? then key 
+    else (
+      reveal_IsPrefix();
+      assume |pset.value.newPrefix + key[|pset.value.prefix|..]| <= 1024;
+      pset.value.newPrefix + key[|pset.value.prefix|..]
+    )
+  }
+
+  function ComposePrefixSet(a: Option<PrefixSet>, b: Option<PrefixSet>): (c: Option<PrefixSet>)
+  requires a.Some? && b.Some? ==> 
+    ( IsPrefix(a.value.prefix, b.value.prefix)
+    || IsPrefix(b.value.prefix, a.value.prefix))
+  {
+    if a == None then (
+      RevPrefixSet(b)
+    ) else if b == None then (
+      a
+    ) else (
+      reveal_IsPrefix();
+      if |a.value.prefix| <= |b.value.prefix| then (
+        var newPrefix := ApplyPrefixSet(a, b.value.prefix);  
+        Some(PrefixSet(b.value.newPrefix, newPrefix))
+      ) else (
+        var prefix := ApplyPrefixSet(b, a.value.prefix);
+        Some(PrefixSet(prefix, a.value.newPrefix))
+      )
+    )
+  }
+
+  lemma ComposePrefixSetCorrect(a: Option<PrefixSet>, b: Option<PrefixSet>, c: Option<PrefixSet>, 
+    key: Key, akey: Key, ckey: Key)
+  requires a.Some? && b.Some? ==> 
+    ( IsPrefix(a.value.prefix, b.value.prefix)
+    || IsPrefix(b.value.prefix, a.value.prefix))
+  requires c == ComposePrefixSet(a, b)
+  requires a.Some? ==> IsPrefix(a.value.prefix, akey)
+  requires b.Some? ==> IsPrefix(b.value.prefix, akey)
+  requires c.Some? ==> IsPrefix(c.value.prefix, ckey)
+  requires a == c ==> akey == ckey
+  requires key == ApplyPrefixSet(a, akey)
+  ensures ApplyPrefixSet(b, akey) == ckey ==> key == ApplyPrefixSet(c, ckey)
+  ensures key == ApplyPrefixSet(c, ckey) ==> ApplyPrefixSet(b, akey) == ckey
+  {
+    reveal_IsPrefix();
+  }
+
+  // given a prefix find its upperbound s.t. lcp(prefix, upper) == prefix
+  function {:opaque} ShortestUncommonPrefix(prefix: Key, idx: int): (upper: Element)
+  requires 0 <= idx <= |prefix|
+  requires forall i | idx < i < |prefix| :: prefix[i] as int == (Uint8UpperBound() as int - 1)
+  ensures upper.Element? ==> (
+    && ElementIsKey(upper)
+    && lcp(prefix, upper.e) == prefix
+    && SeqComparison.lt(prefix, upper.e)
+    && (|upper.e| <= |prefix|)
+    && (upper.e[..|upper.e|-1] == prefix[..|upper.e|-1])
+    && (upper.e[|upper.e|-1] as int == prefix[|upper.e|-1] as int + 1)
+  )
+  ensures PivotLcp(KeyToElement(prefix), upper) == prefix
+  decreases idx
+  {
+    reveal_IsPrefix();
+    SeqComparison.reveal_lte();
+
+    if idx < |prefix| && prefix[idx] as int < Uint8UpperBound() as int - 1
+    then (
+      var k : Key := prefix[..idx] + [prefix[idx] + 1];
+      PrefixLteProperties(prefix[..idx], prefix, k);
+      prefixIslcp(prefix, k);
+      KeyToElement(k)
+    ) else (
+      if idx == 0 then (
+        prefixIslcpright(prefix);
+        Keyspace.Max_Element
+      ) else (
+        ShortestUncommonPrefix(prefix, idx - 1)
+      )
+    )
+  }
+
+  lemma prefixIslcpright(prefix: Key)
+  requires forall i | 0 <= i < |prefix| :: prefix[i] as int == (Uint8UpperBound() as int - 1)
+  ensures lcpright(prefix) == prefix
+  {
+    if |prefix| > 0 {
+      prefixIslcpright(prefix[1..]);
+    }
+  }
+
+  lemma prefixIslcp(prefix: Key, upper: Key)
+  requires 0 < |upper| <= |prefix|
+  requires IsPrefix(prefix[..|upper|-1], upper)
+  requires upper[|upper|-1] as int == (prefix[|upper|-1] as int + 1)
+  requires forall i | |upper| <= i < |prefix| :: prefix[i] as int == (Uint8UpperBound() as int - 1)
+  ensures lcp(prefix, upper) == prefix
+  {
+    reveal_IsPrefix();
+
+    if |upper| == 1 {
+      prefixIslcpright(prefix[1..]);
+    } else {
+      prefixIslcp(prefix[1..], upper[1..]);
+    }
+  }
+
+  lemma PrefixLteProperties(prefix: Key, left: Key, right: Key)
+  requires IsPrefix(prefix, left)
+  requires IsPrefix(prefix, right)
+  ensures SeqComparison.lte(left, right) ==> 
+    ( && SeqComparison.lte(left[|prefix|..], right[|prefix|..])
+      && IsPrefix(prefix, lcp(left, right)))
+  ensures SeqComparison.lte(left[|prefix|..], right[|prefix|..]) ==>
+    ( && SeqComparison.lte(left, right))
+  {
+    reveal_IsPrefix();
+    SeqComparison.reveal_lte();
+
+    if |prefix| > 0 {
+      PrefixLteProperties(prefix[1..], left[1..], right[1..]);
+    }
+  }
+
+  function TranslateElement(e: Element, prefix: Key, newPrefix: Key): (e': Element)
+  requires ElementIsKey(e)
+  requires IsPrefix(prefix, e.e)
+  ensures ElementIsKey(e')
+  ensures IsPrefix(newPrefix, e'.e)
+  {
+    reveal_IsPrefix();
+    var key : Key := e.e;
+    assume |newPrefix + key[|prefix|..]| <= 1024;
+    var translatedKey : Key := newPrefix + key[|prefix|..];
+    KeyToElement(translatedKey)
+  }
+
+  function TranslatePivotPair(pt: PivotTable, et: EdgeTable, slot: int) : (p: (Element, Element))
+  requires WFPivots(pt)
+  requires WFEdges(et, pt)
+  requires 0 <= slot < NumBuckets(pt)
+  requires et[slot].Some?
+  {
+    Keyspace.reveal_IsStrictlySorted();
+
+    var prefix := PivotLcp(pt[slot], pt[slot+1]);
+    var newPrefix := et[slot].value;
+
+    TranslatePivotPairInternal(pt[slot], pt[slot+1], prefix, newPrefix)
+  }
+
+  function TranslatePivotPairInternal(left: Element, right: Element, prefix: Key, newPrefix: Key) : (p: (Element, Element))
+  requires ElementIsKey(left)
+  requires right.Element? ==> ElementIsKey(right)
+  requires IsPrefix(prefix, left.e)
+  requires Keyspace.lt(left, right)
+  ensures var (left', right') := p;
+        && Keyspace.lt(left', right')
+        && ElementIsKey(left')
+        && (right'.Element? ==> ElementIsKey(right'))
+        && AllKeysInBetweenHasPrefix(left', right', newPrefix)
+  {
+    var left' := TranslateElement(left, prefix, newPrefix);
+
+    if right.Max_Element? || !IsPrefix(prefix, right.e)
+    then (
+      var right' := ShortestUncommonPrefix(newPrefix, |newPrefix|);
+
+      PrefixOfLcpIsPrefixOfKeys(KeyToElement(newPrefix), right', newPrefix);
+      assert Keyspace.lte(KeyToElement(newPrefix), left') by {
+        SeqComparison.reveal_lte();
+        PrefixLteProperties(newPrefix, newPrefix, left'.e);
+      }
+
+      if right'.Max_Element? then (
+        assert Keyspace.lt(left', right');
+        (left', right')
+      ) else (
+        KeyWithPrefixLt(newPrefix, right'.e, left'.e);
+        (left', right')
+      )
+    ) else (
+      var right' := TranslateElement(right, prefix, newPrefix);
+
+      PrefixLteProperties(prefix, left.e, right.e);
+      PrefixLteProperties(newPrefix, left'.e, right'.e);
+      PrefixOfLcpIsPrefixOfKeys(left', right', newPrefix);
+
+      (left', right')
+    )
+  }
+
+  lemma KeyWithPrefixLt(prefix: Key, right: Key, key: Key)
+  requires SeqComparison.lt(prefix, right)
+  requires IsPrefix(prefix, key)
+  requires !IsPrefix(prefix, right)
+  ensures SeqComparison.lt(key, right)
+  {
+    reveal_IsPrefix();
+    SeqComparison.reveal_lte();
+
+    if |right| > 0 && right[0] == prefix[0] {
+      KeyWithPrefixLt(prefix[1..], right[1..], key[1..]);
+    }
+  }
+
+  lemma AllKeysWithPrefixLt(prefix: Key, right: Key)
+  requires SeqComparison.lt(prefix, right)
+  requires !IsPrefix(prefix, right)
+  ensures forall k : Key | IsPrefix(prefix, k) :: SeqComparison.lt(k, right)
+  {
+    forall k : Key | IsPrefix(prefix, k)
+    ensures SeqComparison.lt(k, right) 
+    {
+      KeyWithPrefixLt(prefix, right, k);
+    }
+  }
+
+  lemma KeyLtPrefix(prefix: Key, key: Key)
+  requires SeqComparison.lt(key, prefix)
+  ensures !IsPrefix(prefix, key)
+  {
+    reveal_IsPrefix();
+    SeqComparison.reveal_lte();
+
+    if |key| > 0 && key[0] == prefix[0] {
+      KeyLtPrefix(prefix[1..], key[1..]);
+    }
+  }
+
+  lemma AllKeysLtPrefix(prefix: Key)
+  ensures forall k : Key | SeqComparison.lt(k, prefix) :: !IsPrefix(prefix, k)
+  {
+    forall k : Key | SeqComparison.lt(k, prefix)
+    ensures !IsPrefix(prefix, k) 
+    {
+      KeyLtPrefix(prefix, k);
+    }
+  }
+
+  lemma TranslatePivotPairRangeProperty(left: Element, right: Element, prefix: Key, newPrefix: Key)
+  requires ElementIsKey(left)
+  requires right.Element? ==> ElementIsKey(right)
+  requires IsPrefix(prefix, left.e)
+  requires Keyspace.lt(left, right)
+  ensures var (left', right') := TranslatePivotPairInternal(left, right, prefix, newPrefix);
+      && (forall k : Key | InBetween(left', right', k) ::
+          && Keyspace.lte(left, Keyspace.Element(prefix + k[|newPrefix|..]))
+          && Keyspace.lt(Keyspace.Element(prefix + k[|newPrefix|..]), right))
+       && (forall k : Key | InBetween(left, right, k) && IsPrefix(prefix, k) ::
+          && Keyspace.lte(left', Keyspace.Element(newPrefix + k[|prefix|..]))
+          && Keyspace.lt(Keyspace.Element(newPrefix + k[|prefix|..]), right'))
+  {
+    var (left', right') := TranslatePivotPairInternal(left, right, prefix, newPrefix);
+
+    forall k : Key | InBetween(left', right', k)
+    ensures Keyspace.lte(left, Keyspace.Element(prefix + k[|newPrefix|..]))
+    ensures Keyspace.lt(Keyspace.Element(prefix + k[|newPrefix|..]), right)
+    {
+      assert IsPrefix(newPrefix, k);
+      assume |prefix + k[|newPrefix|..]| <= 1024;
+      var k' : Key := prefix + k[|newPrefix|..];
+
+      PrefixLteProperties(newPrefix, left'.e, k);
+      PrefixLteProperties(prefix, left.e, k');
+
+      if right.Max_Element? || !IsPrefix(prefix, right.e){
+        if right.Max_Element? {
+          assert Keyspace.lt(Keyspace.Element(k'), right);
+        } else {
+          assert Keyspace.lte(KeyToElement(prefix), left) by {
+            SeqComparison.reveal_lte();
+            PrefixLteProperties(prefix, prefix, left.e);
+          }
+          Keyspace.transitivity_le_lt(KeyToElement(prefix), left, right);
+          assert Keyspace.lt(KeyToElement(prefix), right);
+          KeyWithPrefixLt(prefix, right.e, k');
+        }
+      } else {
+        PrefixLteProperties(newPrefix, k, right'.e);
+        PrefixLteProperties(prefix, k', right.e);
+      }
+    }
+
+    forall k : Key | InBetween(left, right, k) && IsPrefix(prefix, k) 
+    ensures Keyspace.lte(left', Keyspace.Element(newPrefix + k[|prefix|..]))
+    ensures Keyspace.lt(Keyspace.Element(newPrefix + k[|prefix|..]), right')
+    {
+      assume |newPrefix + k[|prefix|..]| <= 1024;
+      var k' : Key := newPrefix + k[|prefix|..];
+
+      PrefixLteProperties(prefix, left.e, k);
+      PrefixLteProperties(newPrefix, left'.e, k');
+
+      if right.Max_Element? || !IsPrefix(prefix, right.e){
+        if right'.Element? {
+          KeyWithPrefixLt(newPrefix, right'.e, k');
+        }
+      } else {
+        PrefixLteProperties(prefix, k, right.e);
+        PrefixLteProperties(newPrefix, k', right'.e);
+      }
+    }
+  }
+
+  function TranslatePivots(pt: PivotTable, prefix: Key, newPrefix: Key, end: Element, idx: int): (pt' : PivotTable)
+  requires WFPivots(pt)
+  requires 0 <= idx < NumBuckets(pt)
+  requires forall i | 0 <= i < NumBuckets(pt) :: IsPrefix(prefix, pt[i].e)
+  requires end.Element? ==> ElementIsKey(end)
+  requires Keyspace.lt(TranslateElement(pt[|pt|-2], prefix, newPrefix), end)
+  ensures WFPivots(pt')
+  ensures |pt'| == |pt[idx..]|
+  ensures forall i | 0 <= i <  NumBuckets(pt') :: 
+      && IsPrefix(newPrefix, pt'[i].e)
+      && pt[idx+i] == TranslateElement(pt'[i], newPrefix, prefix)
+  ensures Last(pt') == end
+  decreases |pt| - idx
+  {
+    reveal_IsPrefix();
+    Keyspace.reveal_IsStrictlySorted();
+
+    if idx + 1 == NumBuckets(pt) then (
+      [ TranslateElement(pt[idx], prefix, newPrefix), end ]
+    ) else (
+      var pt' := [ TranslateElement(pt[idx], prefix, newPrefix) ] + TranslatePivots(pt, prefix, newPrefix, end, idx+1);
+      PrefixLteProperties(prefix, pt[idx].e, pt[idx+1].e);
+      PrefixLteProperties(newPrefix, pt'[0].e, pt'[1].e);
+      pt'
+    )
+  }
+
+  function TranslateEdges(et: EdgeTable, pt: PivotTable, idx: int) : (et': EdgeTable)
+  requires WFPivots(pt)
+  requires WFEdges(et, pt)
+  requires 0 <= idx < |et|
+  ensures |et'| == |et[idx..]|
+  ensures forall i | 0 <= i < |et'| :: et'[i] == 
+    (if et[i+idx].Some? then et[i+idx] else Some(PivotLcp(pt[i+idx], pt[i+idx+1])))
+  decreases |et| - idx
+  {
+    Keyspace.reveal_IsStrictlySorted();
+    var edge := if et[idx].Some? then et[idx] else Some(PivotLcp(pt[idx], pt[idx+1]));
+
+    if idx + 1 == |et| then (
+      [ edge ]
+    ) else (
+      [ edge ] + TranslateEdges(et, pt, idx+1)
+    )
+  }
+
+  lemma TranslatePivotsEdgesPreserveTranslateKey(pt: PivotTable, et: EdgeTable, pt': PivotTable,
+    et': EdgeTable, prefix: Key, newPrefix: Key, end: Element, key: Key, key': Key)
+  requires WFPivots(pt)
+  requires WFPivots(pt')
+  requires |pt| == |pt'|
+  requires WFEdges(et, pt)
+  requires WFEdges(et', pt')
+  requires BoundedKey(pt, key) && IsPrefix(prefix, key)
+  requires BoundedKey(pt', key')
+  requires Route(pt, key) == Route(pt', key')
+  requires key' == newPrefix + key[|prefix|..]
+  requires PivotLcp(pt'[0], Last(pt')) == newPrefix
+  requires forall i | 0 <= i <  NumBuckets(pt') :: 
+      && IsPrefix(newPrefix, pt'[i].e)
+      && pt[i] == TranslateElement(pt'[i], newPrefix, prefix)
+  requires var (_, right) := TranslatePivotPairInternal(pt'[0], Last(pt'), newPrefix, prefix);
+    && right == Last(pt)
+  requires et' == TranslateEdges(et, pt, 0)
+  ensures TranslateKey(pt, et, key) == TranslateKey(pt', et', key')
+  {
+    var i := Route(pt, key);
+    var lcp : Key := PivotLcp(pt[i], pt[i+1]);
+    var lcp' : Key := PivotLcp(pt'[i], pt'[i+1]);
+
+    Keyspace.reveal_IsStrictlySorted();
+    PrefixOfLcpIsPrefixOfKey(pt[i], pt[i+1], lcp, key);
+    PrefixOfLcpIsPrefixOfKey(pt'[i], pt'[i+1], lcp', key');
+
+    if i+1 == NumBuckets(pt') {
+      if pt'[i+1].Max_Element? || !IsPrefix(newPrefix, pt'[i+1].e) {
+        assert PivotLcp(KeyToElement(prefix), Last(pt)) == prefix;
+
+        var lkey : Key := pt[i].e;
+        assert prefix[|prefix|..] == [];
+        Lexi.EmptyLte(lkey[|prefix|..]);
+        PrefixLteProperties(prefix, prefix, lkey);
+        PivotLcpSubRangeRight(KeyToElement(prefix), pt[i], pt[i+1]);
+        assert IsPrefix(prefix, lcp);
+
+        PivotLcpSubRangeRight(pt'[0], pt'[i], pt'[i+1]);
+        assert IsPrefix(newPrefix, lcp');
+
+        if pt'[i+1].Max_Element? && pt[i+1].Max_Element? {
+          SameLcprightSubfix(pt[i].e, prefix, pt'[i].e, newPrefix);
+        } else if pt'[i+1].Max_Element? {
+          SameLcpLcprightSubfix(pt'[i].e, newPrefix, pt[i].e, pt[i+1].e, prefix);
+        } else if pt[i+1].Max_Element? {
+          SameLcpLcprightSubfix(pt[i].e, prefix, pt'[i].e, pt'[i+1].e, newPrefix);
+        } else {
+          SameLcpLcpSubfix(pt[i].e, pt[i+1].e, prefix, pt'[i].e, pt'[i+1].e, newPrefix);
+        }
+      } else {
+        SameLcpSubfix(pt[i].e, pt[i+1].e, prefix, pt'[i].e, pt'[i+1].e, newPrefix);
+      }
+    } else {
+      SameLcpSubfix(pt[i].e, pt[i+1].e, prefix, pt'[i].e, pt'[i+1].e, newPrefix);
+    }
+
+    if et[i].Some? {
+      assert et[i] == et'[i];
+    } else {
+      assert et'[i].value == lcp;
+    }
+  }
+
+  lemma TranslatePivotsSameRoute(pt: PivotTable, pt': PivotTable, prefix: Key, prefix': Key, key: Key, key': Key)
+  requires WFPivots(pt)
+  requires WFPivots(pt')
+  requires |pt| == |pt'|
+  requires BoundedKey(pt, key) && IsPrefix(prefix, key)
+  requires key' == prefix' + key[|prefix|..]
+  requires forall i | 0 <= i <  NumBuckets(pt') :: 
+      && IsPrefix(prefix', pt'[i].e)
+      && pt[i] == TranslateElement(pt'[i], prefix', prefix)
+  requires Keyspace.lt(KeyToElement(key'), Last(pt'))
+  ensures BoundedKey(pt', key')
+  ensures Route(pt, key) == Route(pt', key')
+  {
+    var i := Route(pt, key);
+
+    PrefixLteProperties(prefix, pt[i].e, key);
+    PrefixLteProperties(prefix', pt'[i].e, key');
+
+    if i+1 < NumBuckets(pt) {
+      PrefixLteProperties(prefix, key, pt[i+1].e);
+      PrefixLteProperties(prefix', key', pt'[i+1].e);
+    }
+
+    RouteIs(pt', key', i);
+  }
+
+  // translated bucket and idxs of corresponding keys
+  datatype TBucket = TBucket(b: Bucket, ghost idxs: seq<int>)
+
+  predicate {:opaque} WFTBucket(bucket: Bucket, tbucket: TBucket, prefix: Key, tPrefix: Key, idx: int)
+  requires 0 <= idx <= |bucket.keys|
+  {
+    && PreWFBucket(bucket)
+    && PreWFBucket(tbucket.b)
+    && |tbucket.b.keys| <= |bucket.keys[idx..]|
+    && |tbucket.b.keys| == |tbucket.idxs|
+    && (forall i | 0 <= i < |tbucket.b.keys| ::
+        && idx <= tbucket.idxs[i] < |bucket.keys|
+        && var tkey : Key := tbucket.b.keys[i];
+        && var key : Key := bucket.keys[tbucket.idxs[i]];
+        && IsPrefix(prefix, key)
+        && tkey == ApplyPrefixSet(Some(PrefixSet(prefix, tPrefix)), key)
+        && bucket.msgs[tbucket.idxs[i]] == tbucket.b.msgs[i])
+    && (forall i, j | 0 <= i < j < |tbucket.idxs| :: tbucket.idxs[i] < tbucket.idxs[j])
+    && (forall i | idx <= i < |bucket.keys| && i !in tbucket.idxs :: !IsPrefix(prefix, bucket.keys[i]))
+  }
+
+  function TranslateBucketInternal(bucket: Bucket, prefix: Key, newPrefix: Key, idx: int) : (tbucket: TBucket)
+  requires PreWFBucket(bucket)
+  requires 0 <= idx <= |bucket.keys|
+  ensures WFTBucket(bucket, tbucket, prefix, newPrefix, idx) // not ensured
+  ensures BucketWellMarshalled(bucket) ==> BucketWellMarshalled(tbucket.b)
+  decreases |bucket.keys| - idx
+  {
+    reveal_WFTBucket();
+
+    if idx == |bucket.keys| then (
+      TBucket(Bucket([], []), [])
+    ) else (
+      reveal_IsPrefix();
+      if IsPrefix(prefix, bucket.keys[idx]) then (
+        var key : Key := bucket.keys[idx];
+        assume |newPrefix + key[|prefix|..]| <= 1024;
+        var key' : Key := newPrefix + key[|prefix|..];
+
+        var tbucket := TranslateBucketInternal(bucket, prefix, newPrefix, idx + 1);
+        var tbucket' := TBucket(Bucket([key'] + tbucket.b.keys, [bucket.msgs[idx]] + tbucket.b.msgs), [idx] + tbucket.idxs);
+
+        assert BucketWellMarshalled(bucket) ==> BucketWellMarshalled(tbucket'.b) by {
+          if BucketWellMarshalled(bucket) && |tbucket'.b.keys| > 1 {
+            Lexi.IsStrictlySortedImpliesLt(bucket.keys, idx, tbucket.idxs[0]);
+            PrefixLteProperties(prefix, key,  bucket.keys[tbucket.idxs[0]]);
+            PrefixLteProperties(newPrefix, key',  tbucket.b.keys[0]);
+            Lexi.reveal_IsStrictlySorted();
+          }
+        }
+
+        tbucket'
+      ) else (
+        TranslateBucketInternal(bucket, prefix, newPrefix, idx + 1)
+      )
+    )
+  }
+
+  function TranslateBucket(bucket: Bucket, prefix: Key, newPrefix: Key) : (res : Bucket)
+  requires PreWFBucket(bucket)
+  ensures WFBucket(bucket) ==> WFBucket(res)
+  ensures PreWFBucket(res)
+  ensures BucketWellMarshalled(bucket) ==> BucketWellMarshalled(res)
+  {
+    var tbucket := TranslateBucketInternal(bucket, prefix, newPrefix, 0);
+    tbucket.b
+  }
+
+  function TranslateBuckets(blist: BucketList, prefix: Key, newPrefix: Key) : (res : BucketList)
+  requires forall i | 0 <= i < |blist| :: WFBucket(blist[i])
+  ensures |res| == |blist|
+  ensures forall i | 0 <= i < |res| :: 
+      && WFBucket(res[i])
+      && res[i] == TranslateBucket(blist[i], prefix, newPrefix)
+  ensures BucketListWellMarshalled(blist) ==> BucketListWellMarshalled(res)
+  {
+    if |blist| > 0 then (
+      var newbucket := TranslateBucket(Last(blist), prefix, newPrefix);
+      TranslateBuckets(DropLast(blist), prefix, newPrefix) + [ newbucket ]
+    ) else (
+      blist
+    )
+  }
+
+  lemma TranslateBucketSameMessage(bucket: Bucket, bucket': Bucket, 
+    prefix: Key, newPrefix: Key, key: Key, key': Key)
+  requires WFBucket(bucket)
+  requires WFBucket(bucket')
+  requires BucketWellMarshalled(bucket)
+  requires bucket' == TranslateBucket(bucket, prefix, newPrefix)
+  requires IsPrefix(prefix, key)
+  requires key' == newPrefix + key[|prefix|..]
+  ensures key in bucket.as_map() <==> key' in bucket'.as_map()
+  ensures key in bucket.as_map() ==> (bucket.as_map()[key] == bucket'.as_map()[key'])
+  {
+    var tbucket := TranslateBucketInternal(bucket, prefix, newPrefix, 0);
+    assert tbucket.b == bucket';
+
+    key_sets_eq(bucket.keys, bucket.msgs);
+    key_sets_eq(bucket'.keys, bucket'.msgs);
+
+    reveal_IsPrefix();
+    if key' in bucket'.keys {
+      var i' := GetIndex(bucket'.keys, bucket'.msgs, key');
+      var i := tbucket.idxs[i'];
+
+      assert bucket.keys[i] == key;
+      assert bucket'.keys[i'] == key';
+
+      MapMapsIndex(bucket.keys, bucket.msgs, i);
+      MapMapsIndex(bucket'.keys, bucket'.msgs, i');
+    } else {
+      if key in bucket.keys {
+        var i := GetIndex(bucket.keys, bucket.msgs, key);
+        if i in tbucket.idxs {
+          var i' :| 0 <= i' < |tbucket.idxs| && tbucket.idxs[i'] == i;
+          assert bucket'.keys[i'] == key';
+        }
+        assert false;
+      }
+    }
+  }
+
+  lemma SameLcpSubfix(left: Key, right: Key, prefix: Key, left': Key, right': Key, prefix': Key)
+  requires IsPrefix(prefix, left) && IsPrefix(prefix, right)
+  requires IsPrefix(prefix', left') && IsPrefix(prefix', right')
+  requires left[|prefix|..] == left'[|prefix'|..]
+  requires right[|prefix|..] == right'[|prefix'|..]
+  ensures var Lcp : Key := lcp(left, right);
+    && var Lcp' : Key := lcp(left', right');
+    && IsPrefix(prefix, Lcp)
+    && IsPrefix(prefix', Lcp')
+    && Lcp[|prefix|..] == Lcp'[|prefix'|..]
+  {
+    reveal_IsPrefix();
+    SeqComparison.reveal_lte();
+
+    if |prefix| > 0 && |prefix'| > 0 {
+      SameLcpSubfix(left[1..], right[1..], prefix[1..], left'[1..], right'[1..], prefix'[1..]);
+    } else if |prefix| == 0 && |prefix'| > 0 {
+      SameLcpSubfix(left, right, prefix, left'[1..], right'[1..], prefix'[1..]);
+    } else if |prefix| > 0 && |prefix'| == 0 {
+      SameLcpSubfix(left[1..], right[1..], prefix[1..], left', right', prefix');
+    }
+  }
+
+  lemma SameLcprightSubfix(left: Key, prefix: Key, left': Key, prefix': Key)
+  requires IsPrefix(prefix, left)
+  requires IsPrefix(prefix', left')
+  requires left[|prefix|..] == left'[|prefix'|..]
+  requires IsPrefix(prefix, lcpright(left))
+  requires IsPrefix(prefix', lcpright(left'))
+  ensures var Lcp : Key := lcpright(left);
+    && var Lcp' : Key := lcpright(left');
+    && Lcp[|prefix|..] == Lcp'[|prefix'|..]
+  {
+    reveal_IsPrefix();
+    SeqComparison.reveal_lte();
+
+    if |prefix| > 0 && |prefix'| > 0 {
+      SameLcprightSubfix(left[1..], prefix[1..], left'[1..], prefix'[1..]);
+    } else if |prefix| == 0 && |prefix'| > 0 {
+      SameLcprightSubfix(left, prefix, left'[1..], prefix'[1..]);
+    } else if |prefix| > 0 && |prefix'| == 0 {
+      SameLcprightSubfix(left[1..], prefix[1..], left', prefix');
+    }
+  }
+
+  lemma SameLcpLcprightSubfix(left: Key, prefix: Key, left': Key, right': Key, prefix': Key)
+  requires IsPrefix(prefix, left)
+  requires IsPrefix(prefix', left')
+  requires left[|prefix|..] == left'[|prefix'|..]
+  requires !IsPrefix(prefix', right')
+  requires SeqComparison.lt(left', right')
+  requires IsPrefix(prefix, lcpright(left))
+  requires IsPrefix(prefix', lcp(left', right'))
+  ensures var Lcp : Key := lcpright(left);
+    && var Lcp' : Key := lcp(left', right');
+    && Lcp[|prefix|..] == Lcp'[|prefix'|..]
+  {
+    reveal_IsPrefix();
+    SeqComparison.reveal_lte();
+
+    if |prefix'| > 0 {
+      var newleft := if |prefix| > 0 then left[1..] else left;
+      var newprefix := if |prefix| > 0 then prefix[1..] else prefix;
+
+      if |right'| > 0 && prefix'[0] == right'[0] {
+        SameLcpLcprightSubfix(newleft, newprefix, left'[1..], right'[1..], prefix'[1..]);
+      } else {
+        SameLcprightSubfix(newleft, newprefix, left'[1..], prefix'[1..]);
+      }
+    }
+  }
+
+  lemma SameLcpLcpSubfix(left: Key, right: Key, prefix: Key, left': Key, right': Key, prefix': Key)
+  requires IsPrefix(prefix, left)
+  requires IsPrefix(prefix', left')
+  requires left[|prefix|..] == left'[|prefix'|..]
+  requires !IsPrefix(prefix, right)
+  requires !IsPrefix(prefix', right')
+  requires SeqComparison.lt(left, right)
+  requires SeqComparison.lt(left', right')
+  requires IsPrefix(prefix, lcp(left, right))
+  requires IsPrefix(prefix', lcp(left', right'))
+  ensures var Lcp : Key := lcp(left, right);
+    && var Lcp' : Key := lcp(left', right');
+    && Lcp[|prefix|..] == Lcp'[|prefix'|..]
+  {
+    reveal_IsPrefix();
+    SeqComparison.reveal_lte();
+
+    if |prefix| > 0 && |prefix'| > 0 {
+      if |right| > 0 && |right'| > 0 && prefix[0] == right[0] && prefix'[0] == right'[0] {
+        SameLcpLcpSubfix(left[1..], right[1..], prefix[1..], left'[1..], right'[1..], prefix'[1..]);
+      } else if |right| > 0 && prefix[0] == right[0] {
+        SameLcpLcprightSubfix(left'[1..], prefix'[1..], left[1..], right[1..], prefix[1..]);
+      } else if |right'| > 0 && prefix'[0] == right'[0] {
+        SameLcpLcprightSubfix(left[1..], prefix[1..], left'[1..], right'[1..], prefix'[1..]); 
+      } else {
+        SameLcprightSubfix(left[1..], prefix[1..], left'[1..], prefix'[1..]);
+      }
+    }
+  }
+
+  predicate ParentKeysInChildRange(parentpivots: PivotTable, parentedges: EdgeTable, childpivots: PivotTable, slot: int)
+  requires WFPivots(parentpivots)
+  requires WFPivots(childpivots)
+  requires WFEdges(parentedges, parentpivots)
+  requires 0 <= slot < |parentedges|
+  {
+    Keyspace.reveal_IsStrictlySorted();
+    && (parentedges[slot].None? ==> 
+        ContainsRange(childpivots, parentpivots[slot], parentpivots[slot+1]))
+    && (parentedges[slot].Some? ==> 
+        && var (left, right) := TranslatePivotPair(parentpivots, parentedges, slot);
+        && ContainsRange(childpivots, left, right))
+  }
+}
